### Question:
Determine all pairs (a, b) of non-negative integers such that
a + b
2 − p
ab = 1

### Answer:
Problem Statement:

Determine all pairs 
(
𝑎
,
𝑏
)
(a,b) of non-negative integers such that:

(
𝑎
+
𝑏
)
2
−
4
𝑎
𝑏
=
1
(a+b) 
2
 −4ab=1
Initial Brainstorming and Understanding
Alright, let's dive into this problem. We need to find all non-negative integer pairs 
(
𝑎
,
𝑏
)
(a,b) that satisfy the equation:

(
𝑎
+
𝑏
)
2
−
4
𝑎
𝑏
=
1
(a+b) 
2
 −4ab=1
First Thoughts:

The equation involves both squares and products of 
𝑎
a and 
𝑏
b, which hints at possible factoring or simplification.
Since 
𝑎
a and 
𝑏
b are non-negative integers, their values are limited, so checking small cases might reveal a pattern.
The equation resembles the form of a perfect square, which could lead to a neat algebraic identity.
Exploring Different Strategies
I'll explore a few strategies to approach this problem:

Simplify the Equation Algebraically
Test Small Integer Values
Analyze the Equation for Patterns or Identities
Use Mathematical Induction or Proof by Contradiction
Let's start with the first strategy.

Strategy 1: Simplify the Equation Algebraically
Step 1: Expand the Left Side

(
𝑎
+
𝑏
)
2
−
4
𝑎
𝑏
=
1
𝑎
2
+
2
𝑎
𝑏
+
𝑏
2
−
4
𝑎
𝑏
=
1
𝑎
2
−
2
𝑎
𝑏
+
𝑏
2
=
1
(a+b) 
2
 −4ab=1
a 
2
 +2ab+b 
2
 −4ab=1
a 
2
 −2ab+b 
2
 =1
Step 2: Recognize a Perfect Square

Notice that:

𝑎
2
−
2
𝑎
𝑏
+
𝑏
2
=
(
𝑎
−
𝑏
)
2
a 
2
 −2ab+b 
2
 =(a−b) 
2
 
So, the equation simplifies to:

(
𝑎
−
𝑏
)
2
=
1
(a−b) 
2
 =1
Step 3: Solve for 
𝑎
−
𝑏
a−b

Taking square roots on both sides:

𝑎
−
𝑏
=
±
1
a−b=±1
This leads to two cases:

Case 1: 
𝑎
−
𝑏
=
1
a−b=1
Case 2: 
𝑎
−
𝑏
=
−
1
a−b=−1
Strategy 2: Test Small Integer Values
Before finalizing our solution from Strategy 1, let's test small non-negative integer pairs to ensure our algebraic simplification holds.

Testing Case 1: 
𝑎
−
𝑏
=
1
a−b=1

Pair (1, 0):

(
1
+
0
)
2
−
4
(
1
)
(
0
)
=
1
−
0
=
1
✓
(1+0) 
2
 −4(1)(0)=1−0=1✓
Pair (2, 1):

(
2
+
1
)
2
−
4
(
2
)
(
1
)
=
9
−
8
=
1
✓
(2+1) 
2
 −4(2)(1)=9−8=1✓
Pair (3, 2):

(
3
+
2
)
2
−
4
(
3
)
(
2
)
=
25
−
24
=
1
✓
(3+2) 
2
 −4(3)(2)=25−24=1✓
Testing Case 2: 
𝑎
−
𝑏
=
−
1
a−b=−1

Pair (0, 1):

(
0
+
1
)
2
−
4
(
0
)
(
1
)
=
1
−
0
=
1
✓
(0+1) 
2
 −4(0)(1)=1−0=1✓
Pair (1, 2):

(
1
+
2
)
2
−
4
(
1
)
(
2
)
=
9
−
8
=
1
✓
(1+2) 
2
 −4(1)(2)=9−8=1✓
Pair (2, 3):

(
2
+
3
)
2
−
4
(
2
)
(
3
)
=
25
−
24
=
1
✓
(2+3) 
2
 −4(2)(3)=25−24=1✓
Observation: All tested pairs satisfy the original equation, supporting our algebraic simplification.

Strategy 3: Analyze the Equation for Patterns or Identities
From Strategy 1, we deduced that 
(
𝑎
−
𝑏
)
2
=
1
(a−b) 
2
 =1, leading to 
𝑎
−
𝑏
=
±
1
a−b=±1. This implies:

When 
𝑎
−
𝑏
=
1
a−b=1:

𝑎
=
𝑏
+
1
a=b+1
When 
𝑎
−
𝑏
=
−
1
a−b=−1:

𝑎
=
𝑏
−
1
a=b−1
Implications:

For 
𝑎
=
𝑏
+
1
a=b+1: 
𝑏
b can be any non-negative integer, and 
𝑎
a is simply one more than 
𝑏
b.
For 
𝑎
=
𝑏
−
1
a=b−1: 
𝑏
b must be at least 1 (since 
𝑎
a is non-negative), and 
𝑎
a is one less than 
𝑏
b.
General Solution:

(
𝑎
,
𝑏
)
=
{
(
𝑏
+
1
,
𝑏
)
for 
𝑏
≥
0
(
𝑏
−
1
,
𝑏
)
for 
𝑏
≥
1
(a,b)={ 
(b+1,b)
(b−1,b)
​
  
for b≥0
for b≥1
​
 
This neatly captures all non-negative integer solutions.

Strategy 4: Use Mathematical Induction or Proof by Contradiction
Given that our previous strategies have consistently led us to the same conclusion, induction might seem redundant. However, to solidify our understanding, let's briefly consider an inductive approach.

Base Case: 
𝑏
=
0
b=0

(
𝑎
,
𝑏
)
=
(
1
,
0
)
as derived from 
𝑎
=
𝑏
+
1
(a,b)=(1,0)as derived from a=b+1
(
1
+
0
)
2
−
4
(
1
)
(
0
)
=
1
−
0
=
1
✓
(1+0) 
2
 −4(1)(0)=1−0=1✓
Inductive Step:

Assume that for some 
𝑏
=
𝑘
b=k, the pair 
(
𝑘
+
1
,
𝑘
)
(k+1,k) satisfies the equation.

(
𝑎
+
𝑏
)
2
−
4
𝑎
𝑏
=
(
𝑘
+
1
+
𝑘
)
2
−
4
(
𝑘
+
1
)
𝑘
=
(
2
𝑘
+
1
)
2
−
4
𝑘
(
𝑘
+
1
)
=
4
𝑘
2
+
4
𝑘
+
1
−
4
𝑘
2
−
4
𝑘
=
1
✓
(a+b) 
2
 −4ab=(k+1+k) 
2
 −4(k+1)k=(2k+1) 
2
 −4k(k+1)
=4k 
2
 +4k+1−4k 
2
 −4k=1✓
Similarly, for 
𝑎
=
𝑘
−
1
a=k−1 and 
𝑏
=
𝑘
b=k (where 
𝑘
≥
1
k≥1):

(
𝑎
+
𝑏
)
2
−
4
𝑎
𝑏
=
(
𝑘
−
1
+
𝑘
)
2
−
4
(
𝑘
−
1
)
𝑘
=
(
2
𝑘
−
1
)
2
−
4
𝑘
(
𝑘
−
1
)
=
4
𝑘
2
−
4
𝑘
+
1
−
4
𝑘
2
+
4
𝑘
=
1
✓
(a+b) 
2
 −4ab=(k−1+k) 
2
 −4(k−1)k=(2k−1) 
2
 −4k(k−1)
=4k 
2
 −4k+1−4k 
2
 +4k=1✓
Conclusion of Induction:

By induction, all pairs 
(
𝑏
+
1
,
𝑏
)
(b+1,b) and 
(
𝑏
−
1
,
𝑏
)
(b−1,b) satisfy the equation for all valid non-negative integers 
𝑏
b.

Reflection on the Approach and Potential Mistakes
Initially, I considered expanding the equation and recognizing it as a perfect square, which led me directly to 
(
𝑎
−
𝑏
)
2
=
1
(a−b) 
2
 =1. This simplification was crucial in identifying the relationship between 
𝑎
a and 
𝑏
b.

Potential Mistake:

At first glance, one might overlook the perfect square and attempt more complicated factoring or testing, which can lead to unnecessary complexity. However, recognizing patterns and familiar algebraic identities streamlined the process.

Another Reflection:

While testing small values provided confirmation, it's essential to ensure that the general solution derived algebraically holds for all non-negative integers. Induction served as an additional verification step, reinforcing the validity of the solution.

Final Answer
All pairs 
(
𝑎
,
𝑏
)
(a,b) of non-negative integers that satisfy the equation 
(
𝑎
+
𝑏
)
2
−
4
𝑎
𝑏
=
1
(a+b) 
2
 −4ab=1 are those where:

∣
𝑎
−
𝑏
∣
=
1
∣a−b∣=1
Formally, the solutions are:

(
𝑎
,
𝑏
)
=
{
(
𝑏
+
1
,
𝑏
)
for all 
𝑏
≥
0
(
𝑏
−
1
,
𝑏
)
for all 
𝑏
≥
1
(a,b)={ 
(b+1,b)
(b−1,b)
​
  
for all b≥0
for all b≥1
​
 
Summary of the Thought Process
Simplification: Recognized the equation as a perfect square, leading to a straightforward relationship between 
𝑎
a and 
𝑏
b.
Verification: Tested small integer pairs to confirm the validity of the algebraic solution.
Generalization: Derived a general form for all solutions based on the simplified equation.
Induction: Used mathematical induction to ensure the solution holds for all non-negative integers.
Reflection: Identified and corrected potential oversights, ensuring a robust and complete solution.
By systematically exploring different strategies and verifying each step, we arrived confidently at the complete set of solutions.