### Question:
Define the sequence A1, A2, A3,... by A1 = 1 and for n = 1, 2, 3,...
An+1 = An + 2
An + 1.
Define the sequence B1, B2, B3,... by B1 = 1 and for n = 1, 2, 3,...
Bn+1 = B2
n + 2
2Bn
.
Prove that Bn+1 = A2n for all non-negative integers n.

### Answer:
Problem Statement:

Define the sequences 
𝐴
1
,
𝐴
2
,
𝐴
3
,
…
A 
1
​
 ,A 
2
​
 ,A 
3
​
 ,… and 
𝐵
1
,
𝐵
2
,
𝐵
3
,
…
B 
1
​
 ,B 
2
​
 ,B 
3
​
 ,… as follows:

Sequence A:

𝐴
1
=
1
A 
1
​
 =1
For 
𝑛
=
1
,
2
,
3
,
…
n=1,2,3,…,
𝐴
𝑛
+
1
=
𝐴
𝑛
+
2
𝐴
𝑛
+
1
A 
n+1
​
 = 
A 
n
​
 +1
A 
n
​
 +2
​
 
Sequence B:

𝐵
1
=
1
B 
1
​
 =1
For 
𝑛
=
1
,
2
,
3
,
…
n=1,2,3,…,
𝐵
𝑛
+
1
=
𝐵
𝑛
+
2
2
𝐵
𝑛
B 
n+1
​
 = 
2B 
n
​
 
B 
n
​
 +2
​
 
Objective: Prove that 
𝐵
𝑛
+
1
=
𝐴
2
𝑛
B 
n+1
​
 =A 
2n
​
  for all non-negative integers 
𝑛
n.

Initial Brainstorming and Understanding
Alright, let's tackle this problem step by step. The goal is to establish a relationship between the sequences 
𝐴
A and 
𝐵
B, specifically proving that 
𝐵
𝑛
+
1
=
𝐴
2
𝑛
B 
n+1
​
 =A 
2n
​
  for all non-negative integers 
𝑛
n.

Key Observations:

Recursive Definitions: Both sequences are defined recursively, meaning each term depends on the previous term(s).
Starting Point: Both sequences start with 
𝐴
1
=
𝐵
1
=
1
A 
1
​
 =B 
1
​
 =1.
Objective Relationship: The relationship 
𝐵
𝑛
+
1
=
𝐴
2
𝑛
B 
n+1
​
 =A 
2n
​
  suggests a deep connection between the two sequences, potentially involving indexing and the behavior of the recursive formulas.
Before diving into formal proofs, it might be helpful to compute the first few terms of both sequences to observe any patterns or verify the proposed relationship.

Exploring Different Strategies
I'll explore several strategies to approach this problem:

Compute Initial Terms: Calculate the first few terms of both sequences to verify the relationship.
Mathematical Induction: Use induction to prove that if the relationship holds for a particular 
𝑛
n, it holds for 
𝑛
+
1
n+1.
Analyze Recurrence Relations: Study the recursive formulas to find closed-form expressions or identify inherent patterns.
Seek Alternate Relationships: If the initial relationship doesn't hold, explore if a different relationship exists between sequences 
𝐴
A and 
𝐵
B.
Let's start by computing the initial terms.

Strategy 1: Compute Initial Terms
Calculating Sequence A:

Given:

𝐴
𝑛
+
1
=
𝐴
𝑛
+
2
𝐴
𝑛
+
1
A 
n+1
​
 = 
A 
n
​
 +1
A 
n
​
 +2
​
 
and 
𝐴
1
=
1
A 
1
​
 =1,

𝐴
2
A 
2
​
 :

𝐴
2
=
1
+
2
1
+
1
=
3
2
=
1.5
A 
2
​
 = 
1+1
1+2
​
 = 
2
3
​
 =1.5
𝐴
3
A 
3
​
 :

𝐴
3
=
1.5
+
2
1.5
+
1
=
3.5
2.5
=
1.4
A 
3
​
 = 
1.5+1
1.5+2
​
 = 
2.5
3.5
​
 =1.4
𝐴
4
A 
4
​
 :

𝐴
4
=
1.4
+
2
1.4
+
1
=
3.4
2.4
≈
1.4167
A 
4
​
 = 
1.4+1
1.4+2
​
 = 
2.4
3.4
​
 ≈1.4167
𝐴
5
A 
5
​
 :

𝐴
5
=
1.4167
+
2
1.4167
+
1
≈
3.4167
2.4167
≈
1.4142
A 
5
​
 = 
1.4167+1
1.4167+2
​
 ≈ 
2.4167
3.4167
​
 ≈1.4142
𝐴
6
A 
6
​
 :

𝐴
6
=
1.4142
+
2
1.4142
+
1
≈
3.4142
2.4142
≈
1.4142
A 
6
​
 = 
1.4142+1
1.4142+2
​
 ≈ 
2.4142
3.4142
​
 ≈1.4142
Observations:

The sequence 
𝐴
A appears to be converging to approximately 
2
2
​
  (
≈
1.4142
≈1.4142).
The terms stabilize around 
2
2
​
  as 
𝑛
n increases.
Calculating Sequence B:

Given:

𝐵
𝑛
+
1
=
𝐵
𝑛
+
2
2
𝐵
𝑛
B 
n+1
​
 = 
2B 
n
​
 
B 
n
​
 +2
​
 
and 
𝐵
1
=
1
B 
1
​
 =1,

𝐵
2
B 
2
​
 :

𝐵
2
=
1
+
2
2
×
1
=
3
2
=
1.5
B 
2
​
 = 
2×1
1+2
​
 = 
2
3
​
 =1.5
𝐵
3
B 
3
​
 :

𝐵
3
=
1.5
+
2
2
×
1.5
=
3.5
3
≈
1.1667
B 
3
​
 = 
2×1.5
1.5+2
​
 = 
3
3.5
​
 ≈1.1667
𝐵
4
B 
4
​
 :

𝐵
4
=
1.1667
+
2
2
×
1.1667
≈
3.1667
2.3334
≈
1.3571
B 
4
​
 = 
2×1.1667
1.1667+2
​
 ≈ 
2.3334
3.1667
​
 ≈1.3571
𝐵
5
B 
5
​
 :

𝐵
5
=
1.3571
+
2
2
×
1.3571
≈
3.3571
2.7142
≈
1.2368
B 
5
​
 = 
2×1.3571
1.3571+2
​
 ≈ 
2.7142
3.3571
​
 ≈1.2368
𝐵
6
B 
6
​
 :

𝐵
6
=
1.2368
+
2
2
×
1.2368
≈
3.2368
2.4736
≈
1.3095
B 
6
​
 = 
2×1.2368
1.2368+2
​
 ≈ 
2.4736
3.2368
​
 ≈1.3095
Observations:

Sequence 
𝐵
B exhibits oscillatory behavior, approaching a fixed point.
The terms fluctuate around approximately 
1.28
1.28.
Verification of the Proposed Relationship:

Let's check if 
𝐵
𝑛
+
1
=
𝐴
2
𝑛
B 
n+1
​
 =A 
2n
​
  holds for the computed terms.

For 
𝑛
=
1
n=1:

𝐵
1
+
1
=
𝐵
2
=
1.5
and
𝐴
2
×
1
=
𝐴
2
=
1.5
(Match)
B 
1+1
​
 =B 
2
​
 =1.5andA 
2×1
​
 =A 
2
​
 =1.5(Match)
For 
𝑛
=
2
n=2:

𝐵
2
+
1
=
𝐵
3
≈
1.1667
and
𝐴
2
×
2
=
𝐴
4
≈
1.4167
(Mismatch)
B 
2+1
​
 =B 
3
​
 ≈1.1667andA 
2×2
​
 =A 
4
​
 ≈1.4167(Mismatch)
For 
𝑛
=
3
n=3:

𝐵
3
+
1
=
𝐵
4
≈
1.3571
and
𝐴
2
×
3
=
𝐴
6
≈
1.4142
(Mismatch)
B 
3+1
​
 =B 
4
​
 ≈1.3571andA 
2×3
​
 =A 
6
​
 ≈1.4142(Mismatch)
Conclusion from Initial Terms:

The relationship 
𝐵
𝑛
+
1
=
𝐴
2
𝑛
B 
n+1
​
 =A 
2n
​
  holds for 
𝑛
=
1
n=1 but fails for 
𝑛
=
2
n=2 and 
𝑛
=
3
n=3.
This discrepancy suggests that either the relationship holds only under specific conditions or there might be an error in the problem's formulation.
Strategy 2: Re-examining the Recursive Definitions
Given that the relationship fails for 
𝑛
≥
2
n≥2, it's essential to revisit the recursive definitions to ensure they've been interpreted correctly.

Original Definitions:

Sequence A:

𝐴
𝑛
+
1
=
𝐴
𝑛
+
2
𝐴
𝑛
+
1.
A 
n+1
​
 =An+2An+1.
Sequence B:

𝐵
𝑛
+
1
=
𝐵
2
𝑛
+
22
𝐵
𝑛
.
B 
n+1
​
 =B2n+22Bn.
Possible Interpretations:

Misplaced Parentheses: Perhaps the intended definitions involve different groupings of terms.

Typographical Errors: The original problem statement might have formatting issues, leading to misinterpretation.

Alternative Interpretation 1:

Sequence A:

𝐴
𝑛
+
1
=
𝐴
𝑛
+
2
𝐴
𝑛
+
1
A 
n+1
​
 = 
A 
n
​
 +1
A 
n
​
 +2
​
 
Sequence B:

𝐵
𝑛
+
1
=
𝐵
𝑛
+
2
2
𝐵
𝑛
B 
n+1
​
 = 
2B 
n
​
 
B 
n
​
 +2
​
 
Alternative Interpretation 2:

Sequence A:

𝐴
𝑛
+
1
=
𝐴
𝑛
+
2
𝐴
𝑛
+
1
A 
n+1
​
 =A 
n
​
 + 
A 
n
​
 +1
2
​
 
Sequence B:

𝐵
𝑛
+
1
=
𝐵
𝑛
+
2
2
𝐵
𝑛
B 
n+1
​
 = 
2B 
n
​
 
B 
n
​
 +2
​
 
Decision:

Given the ambiguity, I'll proceed with the initial, most straightforward interpretation:

Sequence A:

𝐴
𝑛
+
1
=
𝐴
𝑛
+
2
𝐴
𝑛
+
1
A 
n+1
​
 = 
A 
n
​
 +1
A 
n
​
 +2
​
 
Sequence B:

𝐵
𝑛
+
1
=
𝐵
𝑛
+
2
2
𝐵
𝑛
B 
n+1
​
 = 
2B 
n
​
 
B 
n
​
 +2
​
 
Recognizing that the relationship 
𝐵
𝑛
+
1
=
𝐴
2
𝑛
B 
n+1
​
 =A 
2n
​
  doesn't hold universally based on initial terms, I'll explore further to identify any underlying patterns or alternative relationships.

Strategy 3: Analyzing the Behavior of Sequences A and B
Sequence A Analysis:

Given:

𝐴
𝑛
+
1
=
𝐴
𝑛
+
2
𝐴
𝑛
+
1
A 
n+1
​
 = 
A 
n
​
 +1
A 
n
​
 +2
​
 
Fixed Point:

Find 
𝐴
A such that 
𝐴
=
𝐴
+
2
𝐴
+
1
A= 
A+1
A+2
​
 .
Solving:
𝐴
(
𝐴
+
1
)
=
𝐴
+
2
𝐴
2
+
𝐴
=
𝐴
+
2
𝐴
2
=
2
𝐴
=
2
A(A+1)=A+2
A 
2
 +A=A+2
A 
2
 =2
A= 
2
​
 
Conclusion: The sequence 
𝐴
A converges to 
2
2
​
 .
Monotonicity:

Starting with 
𝐴
1
=
1
A 
1
​
 =1:
𝐴
2
=
1.5
>
𝐴
1
A 
2
​
 =1.5>A 
1
​
 
𝐴
3
=
1.4
<
𝐴
2
A 
3
​
 =1.4<A 
2
​
 
𝐴
4
≈
1.4167
>
𝐴
3
A 
4
​
 ≈1.4167>A 
3
​
 
𝐴
5
≈
1.4142
<
𝐴
4
A 
5
​
 ≈1.4142<A 
4
​
 
The sequence oscillates, approaching 
2
2
​
  from both sides.
Sequence B Analysis:

Given:

𝐵
𝑛
+
1
=
𝐵
𝑛
+
2
2
𝐵
𝑛
B 
n+1
​
 = 
2B 
n
​
 
B 
n
​
 +2
​
 
Fixed Point:
Find 
𝐵
B such that 
𝐵
=
𝐵
+
2
2
𝐵
B= 
2B
B+2
​
 .
Solving:
2
𝐵
2
=
𝐵
+
2
2
𝐵
2
−
𝐵
−
2
=
0
𝐵
=
1
±
1
+
16
4
=
1
±
17
4
2B 
2
 =B+2
2B 
2
 −B−2=0
B= 
4
1± 
1+16
​
 
​
 = 
4
1± 
17
​
 
​
 
Positive Root: 
𝐵
=
1
+
17
4
≈
1.2808
B= 
4
1+ 
17
​
 
​
 ≈1.2808
Monotonicity:
Starting with 
𝐵
1
=
1
B 
1
​
 =1:
𝐵
2
=
1.5
>
𝐵
1
B 
2
​
 =1.5>B 
1
​
 
𝐵
3
≈
1.1667
<
𝐵
2
B 
3
​
 ≈1.1667<B 
2
​
 
𝐵
4
≈
1.3571
>
𝐵
3
B 
4
​
 ≈1.3571>B 
3
​
 
𝐵
5
≈
1.2368
<
𝐵
4
B 
5
​
 ≈1.2368<B 
4
​
 
The sequence oscillates, approaching the fixed point 
≈
1.2808
≈1.2808 from both sides.
Comparing Sequences A and B:

Convergence Points:
Sequence 
𝐴
A converges to 
2
≈
1.4142
2
​
 ≈1.4142.
Sequence 
𝐵
B converges to 
1
+
17
4
≈
1.2808
4
1+ 
17
​
 
​
 ≈1.2808.
Oscillatory Behavior:
Both sequences oscillate around their respective fixed points.
Initial Matching:
For 
𝑛
=
1
n=1, 
𝐵
2
=
𝐴
2
=
1.5
B 
2
​
 =A 
2
​
 =1.5.
For 
𝑛
=
2
n=2, 
𝐵
3
≈
1.1667
B 
3
​
 ≈1.1667 vs. 
𝐴
4
≈
1.4167
A 
4
​
 ≈1.4167 (No match).
Conclusion from Analysis:

The relationship 
𝐵
𝑛
+
1
=
𝐴
2
𝑛
B 
n+1
​
 =A 
2n
​
  holds for 
𝑛
=
1
n=1 but fails for 
𝑛
=
2
n=2 and 
𝑛
=
3
n=3. This suggests that the relationship might not hold universally or that there might be an error in the problem's formulation.

Strategy 4: Seeking Alternative Relationships
Given that 
𝐵
𝑛
+
1
=
𝐴
2
𝑛
B 
n+1
​
 =A 
2n
​
  doesn't hold for all 
𝑛
n, I'll explore whether there's another relationship between sequences 
𝐴
A and 
𝐵
B.

Possible Relationships to Explore:

Direct Equality: 
𝐵
𝑛
=
𝐴
𝑛
B 
n
​
 =A 
n
​
  or 
𝐵
𝑛
=
𝐴
𝑛
+
1
B 
n
​
 =A 
n+1
​
 .
Reciprocal Relationship: 
𝐵
𝑛
=
1
𝐴
𝑛
B 
n
​
 = 
A 
n
​
 
1
​
  or similar.
Multiplicative Factors: 
𝐵
𝑛
B 
n
​
  is a multiple of 
𝐴
𝑛
A 
n
​
  or vice versa.
Function Composition: 
𝐵
𝑛
B 
n
​
  is a function of 
𝐴
𝑛
A 
n
​
 .
Testing Direct Equality:

For 
𝑛
=
1
n=1:

𝐵
1
=
1
and
𝐴
1
=
1
(Match)
B 
1
​
 =1andA 
1
​
 =1(Match)
For 
𝑛
=
2
n=2:

𝐵
2
=
1.5
and
𝐴
2
=
1.5
(Match)
B 
2
​
 =1.5andA 
2
​
 =1.5(Match)
For 
𝑛
=
3
n=3:

𝐵
3
≈
1.1667
and
𝐴
3
=
1.4
(Mismatch)
B 
3
​
 ≈1.1667andA 
3
​
 =1.4(Mismatch)
For 
𝑛
=
4
n=4:

𝐵
4
≈
1.3571
and
𝐴
4
≈
1.4167
(Mismatch)
B 
4
​
 ≈1.3571andA 
4
​
 ≈1.4167(Mismatch)
Conclusion:

The relationship 
𝐵
𝑛
=
𝐴
𝑛
B 
n
​
 =A 
n
​
  holds for 
𝑛
=
1
n=1 and 
𝑛
=
2
n=2 but fails for 
𝑛
=
3
n=3 and beyond.

Testing Reciprocal Relationship:

For 
𝑛
=
1
n=1:

𝐵
1
=
1
and
1
𝐴
1
=
1
(Match)
B 
1
​
 =1and 
A 
1
​
 
1
​
 =1(Match)
For 
𝑛
=
2
n=2:

𝐵
2
=
1.5
and
1
𝐴
2
=
1
1.5
≈
0.6667
(Mismatch)
B 
2
​
 =1.5and 
A 
2
​
 
1
​
 = 
1.5
1
​
 ≈0.6667(Mismatch)
Conclusion:

The reciprocal relationship does not hold beyond 
𝑛
=
1
n=1.

Testing Multiplicative Factors:

For 
𝑛
=
1
n=1:

𝐵
1
=
1
=
1
×
𝐴
1
(Match)
B 
1
​
 =1=1×A 
1
​
 (Match)
For 
𝑛
=
2
n=2:

𝐵
2
=
1.5
=
1
×
𝐴
2
(Match)
B 
2
​
 =1.5=1×A 
2
​
 (Match)
For 
𝑛
=
3
n=3:

𝐵
3
≈
1.1667
and
1
×
𝐴
3
=
1.4
(Mismatch)
B 
3
​
 ≈1.1667and1×A 
3
​
 =1.4(Mismatch)
Conclusion:

Multiplicative relationships like 
𝐵
𝑛
=
𝑘
×
𝐴
𝑛
B 
n
​
 =k×A 
n
​
  only hold for the initial terms.

Strategy 5: Revisiting the Problem Statement
Given the inconsistencies found, it's crucial to ensure that the recursive definitions are interpreted correctly. Misinterpretation due to formatting issues can lead to incorrect conclusions.

Original Definitions Revisited:

Sequence A:

𝐴
𝑛
+
1
=
𝐴
𝑛
+
2
𝐴
𝑛
+
1.
A 
n+1
​
 =An+2An+1.
Sequence B:

𝐵
𝑛
+
1
=
𝐵
2
𝑛
+
22
𝐵
𝑛
.
B 
n+1
​
 =B2n+22Bn.
Possible Correct Interpretation:

It's plausible that the intended definitions involve fractions, given the context. Hence:

Sequence A:

𝐴
𝑛
+
1
=
𝐴
𝑛
+
2
𝐴
𝑛
+
1
A 
n+1
​
 = 
A 
n
​
 +1
A 
n
​
 +2
​
 
Sequence B:

𝐵
𝑛
+
1
=
𝐵
𝑛
+
2
2
𝐵
𝑛
B 
n+1
​
 = 
2B 
n
​
 
B 
n
​
 +2
​
 
Assuming this is correct, let's proceed.

Strategy 6: Mathematical Induction
Given the uncertainty in the relationship based on initial terms, mathematical induction might help clarify if the relationship holds beyond the initial terms.

Base Case:

For 
𝑛
=
0
n=0:

𝐵
0
+
1
=
𝐵
1
=
1
and
𝐴
2
×
0
=
𝐴
0
B 
0+1
​
 =B 
1
​
 =1andA 
2×0
​
 =A 
0
​
 
However, 
𝐴
0
A 
0
​
  is not defined in the original problem. To align with the sample solution, let's define 
𝐴
0
=
1
A 
0
​
 =1.

𝐵
1
=
1
=
𝐴
0
=
1
(Match)
B 
1
​
 =1=A 
0
​
 =1(Match)
For 
𝑛
=
1
n=1:

𝐵
1
+
1
=
𝐵
2
=
1.5
and
𝐴
2
×
1
=
𝐴
2
=
1.5
(Match)
B 
1+1
​
 =B 
2
​
 =1.5andA 
2×1
​
 =A 
2
​
 =1.5(Match)
Conclusion: The base cases 
𝑛
=
0
n=0 and 
𝑛
=
1
n=1 hold.

Inductive Step:

Assume that for some 
𝑛
=
𝑘
n=k, 
𝐵
𝑘
+
1
=
𝐴
2
𝑘
B 
k+1
​
 =A 
2k
​
  holds.

We need to prove that 
𝐵
(
𝑘
+
1
)
+
1
=
𝐵
𝑘
+
2
=
𝐴
2
(
𝑘
+
1
)
=
𝐴
2
𝑘
+
2
B 
(k+1)+1
​
 =B 
k+2
​
 =A 
2(k+1)
​
 =A 
2k+2
​
 .

Expressing 
𝐵
𝑘
+
2
B 
k+2
​
 :

𝐵
𝑘
+
2
=
𝐵
𝑘
+
1
+
2
2
𝐵
𝑘
+
1
=
𝐴
2
𝑘
+
2
2
𝐴
2
𝑘
B 
k+2
​
 = 
2B 
k+1
​
 
B 
k+1
​
 +2
​
 = 
2A 
2k
​
 
A 
2k
​
 +2
​
 
Expressing 
𝐴
2
𝑘
+
2
A 
2k+2
​
 :

𝐴
2
𝑘
+
2
=
𝐴
2
𝑘
+
1
+
2
𝐴
2
𝑘
+
1
+
1
A 
2k+2
​
 = 
A 
2k+1
​
 +1
A 
2k+1
​
 +2
​
 
Challenge:

To connect 
𝐵
𝑘
+
2
B 
k+2
​
  with 
𝐴
2
𝑘
+
2
A 
2k+2
​
 , we need an expression for 
𝐴
2
𝑘
+
1
A 
2k+1
​
  in terms of 
𝐴
2
𝑘
A 
2k
​
 .

But, from the recursive definition of 
𝐴
A:

𝐴
2
𝑘
+
1
=
𝐴
2
𝑘
+
2
𝐴
2
𝑘
+
1
A 
2k+1
​
 = 
A 
2k
​
 +1
A 
2k
​
 +2
​
 
Substituting into 
𝐴
2
𝑘
+
2
A 
2k+2
​
 :

A_{2k+2} = \frac{\left( \frac{A_{2k} + 2}{A_{2k} + 1} \right) + 2}{\left( \frac{A_{2k} + 2}{A_{2k} + 1} \right) + 1} = \frac{\frac{A_{2k} + 2 + 2(A_{2k} + 1)}{A_{2k} + 1}}{\frac{A_{2k} + 2 + A_{2k} + 1}{A_{2k} + 1}}} = \frac{A_{2k} + 2 + 2A_{2k} + 2}{2A_{2k} + 3} = \frac{3A_{2k} + 4}{2A_{2k} + 3}
Comparing 
𝐵
𝑘
+
2
B 
k+2
​
  and 
𝐴
2
𝑘
+
2
A 
2k+2
​
 :

𝐵
𝑘
+
2
=
𝐴
2
𝑘
+
2
2
𝐴
2
𝑘
and
𝐴
2
𝑘
+
2
=
3
𝐴
2
𝑘
+
4
2
𝐴
2
𝑘
+
3
B 
k+2
​
 = 
2A 
2k
​
 
A 
2k
​
 +2
​
 andA 
2k+2
​
 = 
2A 
2k
​
 +3
3A 
2k
​
 +4
​
 
To establish 
𝐵
𝑘
+
2
=
𝐴
2
𝑘
+
2
B 
k+2
​
 =A 
2k+2
​
 , we need:

𝐴
2
𝑘
+
2
2
𝐴
2
𝑘
=
3
𝐴
2
𝑘
+
4
2
𝐴
2
𝑘
+
3
2A 
2k
​
 
A 
2k
​
 +2
​
 = 
2A 
2k
​
 +3
3A 
2k
​
 +4
​
 
Cross-Multiplying:

(
𝐴
2
𝑘
+
2
)
(
2
𝐴
2
𝑘
+
3
)
=
2
𝐴
2
𝑘
(
3
𝐴
2
𝑘
+
4
)
(A 
2k
​
 +2)(2A 
2k
​
 +3)=2A 
2k
​
 (3A 
2k
​
 +4)
Expanding both sides:

Left Side:

(
𝐴
2
𝑘
+
2
)
(
2
𝐴
2
𝑘
+
3
)
=
2
𝐴
2
𝑘
2
+
3
𝐴
2
𝑘
+
4
𝐴
2
𝑘
+
6
=
2
𝐴
2
𝑘
2
+
7
𝐴
2
𝑘
+
6
(A 
2k
​
 +2)(2A 
2k
​
 +3)=2A 
2k
2
​
 +3A 
2k
​
 +4A 
2k
​
 +6=2A 
2k
2
​
 +7A 
2k
​
 +6
Right Side:

2
𝐴
2
𝑘
(
3
𝐴
2
𝑘
+
4
)
=
6
𝐴
2
𝑘
2
+
8
𝐴
2
𝑘
2A 
2k
​
 (3A 
2k
​
 +4)=6A 
2k
2
​
 +8A 
2k
​
 
Setting Both Sides Equal:

2
𝐴
2
𝑘
2
+
7
𝐴
2
𝑘
+
6
=
6
𝐴
2
𝑘
2
+
8
𝐴
2
𝑘
2A 
2k
2
​
 +7A 
2k
​
 +6=6A 
2k
2
​
 +8A 
2k
​
 
Rearranging:

0
=
4
𝐴
2
𝑘
2
+
𝐴
2
𝑘
−
6
0=4A 
2k
2
​
 +A 
2k
​
 −6
Solving for 
𝐴
2
𝑘
A 
2k
​
 :

4
𝐴
2
𝑘
2
+
𝐴
2
𝑘
−
6
=
0
𝐴
2
𝑘
=
−
1
±
1
+
96
8
=
−
1
±
97
8
4A 
2k
2
​
 +A 
2k
​
 −6=0
A 
2k
​
 = 
8
−1± 
1+96
​
 
​
 = 
8
−1± 
97
​
 
​
 
Given that 
𝐴
𝑛
A 
n
​
  is always positive, we discard the negative root:

𝐴
2
𝑘
=
−
1
+
97
8
≈
−
1
+
9.849
8
≈
1.106
A 
2k
​
 = 
8
−1+ 
97
​
 
​
 ≈ 
8
−1+9.849
​
 ≈1.106
Comparison with Actual 
𝐴
2
𝑘
A 
2k
​
 :

From our earlier computations:

𝐴
2
=
1.5
A 
2
​
 =1.5
𝐴
4
≈
1.4167
A 
4
​
 ≈1.4167
𝐴
6
≈
1.4142
A 
6
​
 ≈1.4142
But according to the above equation, 
𝐴
2
𝑘
≈
1.106
A 
2k
​
 ≈1.106 when 
𝑘
≥
1
k≥1, which does not align with our computed values. This inconsistency suggests a flaw in our assumption or approach.

Reflection:

The inductive step leads to an equation that contradicts the actual values of 
𝐴
2
𝑘
A 
2k
​
 . This indicates that our initial assumption—that 
𝐵
𝑘
+
1
=
𝐴
2
𝑘
B 
k+1
​
 =A 
2k
​
  holds—might be incorrect beyond the base case. It could also imply that there is an error in our interpretation of the recursive definitions or the intended relationship between sequences 
𝐴
A and 
𝐵
B.

Strategy 7: Seeking a Transformation or Functional Relationship
Perhaps there's a different way to relate sequences 
𝐴
A and 
𝐵
B that isn't immediately apparent.

Possible Transformations:

Reciprocal: 
𝐵
𝑛
=
1
𝐴
𝑛
B 
n
​
 = 
A 
n
​
 
1
​
  or similar.
Multiplicative Factors: 
𝐵
𝑛
B 
n
​
  is a multiple of 
𝐴
𝑛
A 
n
​
  or vice versa.
Function Composition: 
𝐵
𝑛
B 
n
​
  is a function of 
𝐴
𝑛
A 
n
​
 .
Testing Reciprocal Transformation:

For 
𝑛
=
1
n=1:

𝐵
1
=
1
and
1
𝐴
1
=
1
(Match)
B 
1
​
 =1and 
A 
1
​
 
1
​
 =1(Match)
For 
𝑛
=
2
n=2:

𝐵
2
=
1.5
and
1
𝐴
2
=
1
1.5
≈
0.6667
(Mismatch)
B 
2
​
 =1.5and 
A 
2
​
 
1
​
 = 
1.5
1
​
 ≈0.6667(Mismatch)
Conclusion:

The reciprocal relationship does not hold beyond 
𝑛
=
1
n=1.

Testing Linear Combination:

Attempting to find constants 
𝑐
c and 
𝑑
d such that 
𝐵
𝑛
+
1
=
𝑐
×
𝐴
2
𝑛
+
𝑑
B 
n+1
​
 =c×A 
2n
​
 +d.

For 
𝑛
=
1
n=1:

𝐵
2
=
1.5
=
𝑐
×
𝐴
2
+
𝑑
=
𝑐
×
1.5
+
𝑑
B 
2
​
 =1.5=c×A 
2
​
 +d=c×1.5+d
For 
𝑛
=
2
n=2:

𝐵
3
≈
1.1667
=
𝑐
×
𝐴
4
+
𝑑
≈
𝑐
×
1.4167
+
𝑑
B 
3
​
 ≈1.1667=c×A 
4
​
 +d≈c×1.4167+d
Solving the system:

From the first equation:

1.5
=
1.5
𝑐
+
𝑑
⇒
𝑑
=
1.5
−
1.5
𝑐
1.5=1.5c+d⇒d=1.5−1.5c
Substituting into the second equation:

1.1667
=
1.4167
𝑐
+
(
1.5
−
1.5
𝑐
)
1.1667
=
(
1.4167
𝑐
−
1.5
𝑐
)
+
1.5
1.1667
=
−
0.0833
𝑐
+
1.5
−
0.3333
≈
−
0.0833
𝑐
⇒
𝑐
≈
4
1.1667=1.4167c+(1.5−1.5c)
1.1667=(1.4167c−1.5c)+1.5
1.1667=−0.0833c+1.5
−0.3333≈−0.0833c⇒c≈4
Then,

𝑑
=
1.5
−
1.5
×
4
=
1.5
−
6
=
−
4.5
d=1.5−1.5×4=1.5−6=−4.5
Testing with 
𝑐
=
4
c=4 and 
𝑑
=
−
4.5
d=−4.5:

For 
𝑛
=
1
n=1:

𝐵
2
=
1.5
=
4
×
1.5
−
4.5
=
6
−
4.5
=
1.5
(Match)
B 
2
​
 =1.5=4×1.5−4.5=6−4.5=1.5(Match)
For 
𝑛
=
2
n=2:

𝐵
3
≈
1.1667
=
4
×
1.4167
−
4.5
≈
5.6668
−
4.5
=
1.1668
(Match)
B 
3
​
 ≈1.1667=4×1.4167−4.5≈5.6668−4.5=1.1668(Match)
For 
𝑛
=
3
n=3:

𝐵
4
≈
1.3571
=
4
×
1.4142
−
4.5
≈
5.6568
−
4.5
=
1.6568
(Mismatch)
B 
4
​
 ≈1.3571=4×1.4142−4.5≈5.6568−4.5=1.6568(Mismatch)
Conclusion:

The linear combination works for 
𝑛
=
1
n=1 and 
𝑛
=
2
n=2 but fails for 
𝑛
=
3
n=3. This suggests that such a transformation is not universally applicable.

Strategy 8: Abandoning the Proposed Relationship and Seeking Clarification
Given that multiple strategies do not uphold the relationship 
𝐵
𝑛
+
1
=
𝐴
2
𝑛
B 
n+1
​
 =A 
2n
​
  beyond 
𝑛
=
1
n=1, it's reasonable to suspect that there might be an error in the problem statement or its interpretation.

Possible Issues:

Typographical Errors: The original problem statement might have formatting issues, leading to misinterpretation of the recursive formulas.
Incorrect Relationship: The intended relationship between sequences 
𝐴
A and 
𝐵
B might differ from 
𝐵
𝑛
+
1
=
𝐴
2
𝑛
B 
n+1
​
 =A 
2n
​
 .
Additional Constraints: There might be hidden constraints or additional information not provided in the problem statement.
Recommendation:

Before proceeding further, it's advisable to:

Verify the Problem Statement: Ensure that the formulas for 
𝐴
𝑛
+
1
A 
n+1
​
  and 
𝐵
𝑛
+
1
B 
n+1
​
  are correctly interpreted. If possible, refer back to the original source or consult additional materials for clarification.
Re-examine the Intended Relationship: Confirm whether 
𝐵
𝑛
+
1
=
𝐴
2
𝑛
B 
n+1
​
 =A 
2n
​
  is the correct relationship or if another relationship was intended.
Seek Additional Information: Look for examples, hints, or contextual information that might shed light on the correct interpretation.
Final Conclusion
After exploring multiple strategies, including computing initial terms, attempting mathematical induction, and seeking transformations, it becomes evident that the proposed relationship 
𝐵
𝑛
+
1
=
𝐴
2
𝑛
B 
n+1
​
 =A 
2n
​
  does not hold universally for all non-negative integers 
𝑛
n. Specifically, while the relationship holds for 
𝑛
=
1
n=1, it fails for 
𝑛
=
2
n=2 and beyond.

Possible Reasons:

Misinterpretation of Recursive Definitions: The recursive formulas for sequences 
𝐴
A and 
𝐵
B might have been misread due to formatting issues.
Error in the Problem Statement: There might be an error in how the problem was presented, leading to an incorrect relationship.
Alternative Relationship: The intended relationship between sequences 
𝐴
A and 
𝐵
B might be different from what's stated.
Next Steps:

To resolve this discrepancy, I recommend:

Clarifying the Recursive Definitions: Ensure that the formulas for 
𝐴
𝑛
+
1
A 
n+1
​
  and 
𝐵
𝑛
+
1
B 
n+1
​
  are correctly interpreted, possibly involving fractions or different groupings.
Re-evaluating the Relationship: Consider alternative relationships between sequences 
𝐴
A and 
𝐵
B that might hold consistently across all 
𝑛
n.
Consulting Additional Resources: If available, refer to the original problem source or seek examples that demonstrate the relationship.
Reflection and Learning Points
Importance of Clear Definitions: Ambiguities in problem definitions can lead to misinterpretations and incorrect conclusions.
Testing Hypotheses Early: Computing initial terms is a valuable strategy to test the validity of proposed relationships.
Flexibility in Approach: Being open to revisiting and revising strategies is crucial when initial approaches don't yield consistent results.
Error Detection: Identifying inconsistencies early helps in diagnosing potential errors in problem definitions or assumptions.
Final Verdict:

Based on the given definitions and the analysis conducted, the relationship 
𝐵
𝑛
+
1
=
𝐴
2
𝑛
B 
n+1
​
 =A 
2n
​
  does not hold for all non-negative integers 
𝑛
n. To proceed effectively, it's essential to ensure that the sequences are correctly defined and to verify the intended relationship between them.






