### Question:
Let 
n
n be an even positive integer. Let 
p
p be a monic, real polynomial of degree 
2
n
2n; that is to say,

p
(
x
)
=
x
2
n
+
a
2
n
−
1
x
2
n
−
1
+
⋯
+
a
1
x
+
a
0
p(x)=x 
2n
 +a 
2n−1
​
 x 
2n−1
 +⋯+a 
1
​
 x+a 
0
​
 

for some real coefficients 
a
0
,
…
,
a
2
n
−
1
a 
0
​
 ,…,a 
2n−1
​
 . Suppose that 
p
(
1
k
)
=
k
2
p( 
k
1
​
 )=k 
2
  for all integers 
k
k such that 
1
≤
∣
k
∣
≤
n
1≤∣k∣≤n.

Find all other real numbers 
x
x for which 
p
(
1
x
)
=
x
2
p( 
x
1
​
 )=x 
2
 .

### Answer:

Absolutely, let's approach this problem step-by-step, emulating a human's problem-solving journey. We'll explore various strategies, reflect on their effectiveness, and adjust our approach as needed to arrive at the solution.

Problem Statement:

Let 
𝑛
n be an even positive integer.
Let 
𝑝
(
𝑥
)
p(x) be a monic real polynomial of degree 
2
𝑛
2n:
𝑝
(
𝑥
)
=
𝑥
2
𝑛
+
𝑎
2
𝑛
−
1
𝑥
2
𝑛
−
1
+
⋯
+
𝑎
1
𝑥
+
𝑎
0
p(x)=x 
2n
 +a 
2n−1
​
 x 
2n−1
 +⋯+a 
1
​
 x+a 
0
​
 
Given that for all integers 
𝑘
k with 
1
≤
∣
𝑘
∣
≤
𝑛
1≤∣k∣≤n:
𝑝
(
1
𝑘
)
=
𝑘
2
p( 
k
1
​
 )=k 
2
 
Goal: Find all other real numbers 
𝑥
x such that:
𝑝
(
1
𝑥
)
=
𝑥
2
p( 
x
1
​
 )=x 
2
 
Step 1: Understanding the Given Information

Before diving into solving, let's dissect what's provided:

Polynomial Characteristics:

Monic: The leading coefficient of 
𝑝
(
𝑥
)
p(x) is 1.
Degree: The polynomial is of degree 
2
𝑛
2n, implying it has 
2
𝑛
2n roots (real or complex).
Given Conditions:

For each integer 
𝑘
k where 
1
≤
∣
𝑘
∣
≤
𝑛
1≤∣k∣≤n, the polynomial satisfies 
𝑝
(
1
𝑘
)
=
𝑘
2
p( 
k
1
​
 )=k 
2
 .
This provides us with 
2
𝑛
2n distinct points since 
𝑘
k ranges from 
−
𝑛
−n to 
𝑛
n, excluding zero.
Objective:

Determine all real numbers 
𝑥
x (including those outside the given integer range) for which 
𝑝
(
1
𝑥
)
=
𝑥
2
p( 
x
1
​
 )=x 
2
 .
Initial Observations:

The relationship 
𝑝
(
1
𝑘
)
=
𝑘
2
p( 
k
1
​
 )=k 
2
  suggests a symmetry or reciprocal relationship within the polynomial.
Since 
𝑝
(
𝑥
)
p(x) is of degree 
2
𝑛
2n and we have 
2
𝑛
2n data points, the polynomial is uniquely determined by these conditions.
The problem asks for solutions beyond the initially provided 
2
𝑛
2n points, hinting at the existence of additional roots.
Step 2: Brainstorming Potential Strategies

To tackle this problem, let's consider various strategies:

Constructing a New Polynomial:

Define a function based on the given condition 
𝑝
(
1
𝑥
)
−
𝑥
2
p( 
x
1
​
 )−x 
2
  and analyze its roots.
Exploring Polynomial Symmetry:

Investigate if 
𝑝
(
𝑥
)
p(x) exhibits reciprocal symmetry or other symmetric properties.
Utilizing Polynomial Identities:

Apply known polynomial identities or transformations that relate 
𝑝
(
𝑥
)
p(x) and 
𝑝
(
1
𝑥
)
p( 
x
1
​
 ).
Applying Vieta's Formulas:

Use relationships between the roots and coefficients of 
𝑝
(
𝑥
)
p(x) to gain insights.
Substitution Method:

Substitute variables (e.g., 
𝑦
=
1
𝑥
y= 
x
1
​
 ) to simplify the equation.
Choosing a Starting Point:

Given the reciprocal nature of the condition 
𝑝
(
1
𝑥
)
=
𝑥
2
p( 
x
1
​
 )=x 
2
 , constructing a new polynomial seems promising. Let's proceed with this strategy.

Step 3: Implementing Strategy 1 – Constructing a New Polynomial

Defining the Function:

Let's define a new function 
𝐹
(
𝑥
)
F(x) as follows:

𝐹
(
𝑥
)
=
𝑝
(
1
𝑥
)
−
𝑥
2
F(x)=p( 
x
1
​
 )−x 
2
 
Our goal is to find all real numbers 
𝑥
x such that 
𝐹
(
𝑥
)
=
0
F(x)=0.

Analyzing Given Conditions:

From the problem, we know that for each integer 
𝑘
k with 
1
≤
∣
𝑘
∣
≤
𝑛
1≤∣k∣≤n:

𝐹
(
𝑘
)
=
𝑝
(
1
𝑘
)
−
𝑘
2
=
0
F(k)=p( 
k
1
​
 )−k 
2
 =0
This means that 
𝐹
(
𝑥
)
F(x) has zeros at 
𝑥
=
±
1
,
±
2
,
…
,
±
𝑛
x=±1,±2,…,±n.

Observing the Nature of 
𝐹
(
𝑥
)
F(x):

𝑝
(
1
𝑥
)
p( 
x
1
​
 ) introduces negative exponents, making 
𝐹
(
𝑥
)
F(x) a rational function.
To handle this, we'll multiply 
𝐹
(
𝑥
)
F(x) by 
𝑥
2
𝑛
x 
2n
  to eliminate negative exponents, transforming it into a polynomial.
Defining 
𝐺
(
𝑥
)
G(x):

Let’s define:

𝐺
(
𝑥
)
=
𝑥
2
𝑛
⋅
𝐹
(
𝑥
)
=
𝑥
2
𝑛
⋅
𝑝
(
1
𝑥
)
−
𝑥
2
𝑛
+
2
G(x)=x 
2n
 ⋅F(x)=x 
2n
 ⋅p( 
x
1
​
 )−x 
2n+2
 
Now, 
𝐺
(
𝑥
)
G(x) is a polynomial. Let's analyze its degree and roots.

Degree of 
𝐺
(
𝑥
)
G(x):

Since 
𝑝
(
𝑥
)
p(x) is of degree 
2
𝑛
2n, 
𝑝
(
1
𝑥
)
p( 
x
1
​
 ) has terms up to 
𝑥
−
2
𝑛
x 
−2n
 .
Multiplying by 
𝑥
2
𝑛
x 
2n
  converts 
𝑝
(
1
𝑥
)
p( 
x
1
​
 ) into a polynomial of degree 
0
0 (constant) to 
2
𝑛
2n.
Subtracting 
𝑥
2
𝑛
+
2
x 
2n+2
  raises the degree of 
𝐺
(
𝑥
)
G(x) to 
2
𝑛
+
2
2n+2.
Identifying the Zeros of 
𝐺
(
𝑥
)
G(x):

From the given conditions, 
𝐹
(
𝑘
)
=
0
F(k)=0 for 
𝑥
=
±
1
,
±
2
,
…
,
±
𝑛
x=±1,±2,…,±n. Therefore, 
𝐺
(
𝑥
)
G(x) also has zeros at these points.

Step 4: Factoring 
𝐺
(
𝑥
)
G(x)

We have identified 
2
𝑛
2n zeros at 
𝑥
=
±
1
,
±
2
,
…
,
±
𝑛
x=±1,±2,…,±n.

Therefore, 
𝐺
(
𝑥
)
G(x) can be factored as:

𝐺
(
𝑥
)
=
(
𝑥
−
1
)
(
𝑥
+
1
)
(
𝑥
−
2
)
(
𝑥
+
2
)
⋯
(
𝑥
−
𝑛
)
(
𝑥
+
𝑛
)
⋅
𝑟
(
𝑥
)
G(x)=(x−1)(x+1)(x−2)(x+2)⋯(x−n)(x+n)⋅r(x)
Simplify the product of pairs:

(
𝑥
−
𝑘
)
(
𝑥
+
𝑘
)
=
𝑥
2
−
𝑘
2
(x−k)(x+k)=x 
2
 −k 
2
 
Thus,

𝐺
(
𝑥
)
=
∏
𝑘
=
1
𝑛
(
𝑥
2
−
𝑘
2
)
⋅
𝑟
(
𝑥
)
G(x)= 
k=1
∏
n
​
 (x 
2
 −k 
2
 )⋅r(x)
Since 
𝐺
(
𝑥
)
G(x) is of degree 
2
𝑛
+
2
2n+2, and 
∏
𝑘
=
1
𝑛
(
𝑥
2
−
𝑘
2
)
∏ 
k=1
n
​
 (x 
2
 −k 
2
 ) is of degree 
2
𝑛
2n, 
𝑟
(
𝑥
)
r(x) must be a quadratic polynomial:

𝑟
(
𝑥
)
=
𝐴
𝑥
2
+
𝐵
𝑥
+
𝐶
r(x)=Ax 
2
 +Bx+C
Step 5: Determining the Coefficients 
𝐴
,
𝐵
,
𝐶
A,B,C of 
𝑟
(
𝑥
)
r(x)

Our goal is to find 
𝐴
,
𝐵
,
A,B, and 
𝐶
C such that:

𝐺
(
𝑥
)
=
(
∏
𝑘
=
1
𝑛
(
𝑥
2
−
𝑘
2
)
)
(
𝐴
𝑥
2
+
𝐵
𝑥
+
𝐶
)
G(x)=( 
k=1
∏
n
​
 (x 
2
 −k 
2
 ))(Ax 
2
 +Bx+C)
Leading Coefficient (
𝐴
A):

The leading term of 
𝐺
(
𝑥
)
G(x) is 
−
𝑥
2
𝑛
+
2
−x 
2n+2
  (from 
−
𝑥
2
𝑛
+
2
−x 
2n+2
  in the expression of 
𝐺
(
𝑥
)
G(x)).
The leading term of 
∏
𝑘
=
1
𝑛
(
𝑥
2
−
𝑘
2
)
∏ 
k=1
n
​
 (x 
2
 −k 
2
 ) is 
𝑥
2
𝑛
x 
2n
 .
The leading term of 
𝑟
(
𝑥
)
r(x) is 
𝐴
𝑥
2
Ax 
2
 .
Therefore, the leading term of the product is 
𝐴
𝑥
2
𝑛
⋅
𝑥
2
=
𝐴
𝑥
2
𝑛
+
2
Ax 
2n
 ⋅x 
2
 =Ax 
2n+2
 .
Equating the leading coefficients:
𝐴
𝑥
2
𝑛
+
2
=
−
𝑥
2
𝑛
+
2
⇒
𝐴
=
−
1
Ax 
2n+2
 =−x 
2n+2
 ⇒A=−1
Coefficient of 
𝑥
2
𝑛
+
1
x 
2n+1
  (
𝐵
B):

Since 
𝐺
(
𝑥
)
G(x) is constructed from 
𝑝
(
1
𝑥
)
p( 
x
1
​
 ) and 
𝑥
2
𝑛
+
2
x 
2n+2
 , both of which are even functions (symmetric in 
𝑥
x), 
𝐺
(
𝑥
)
G(x) cannot have an odd-degree term.
The 
𝑥
2
𝑛
+
1
x 
2n+1
  term arises from multiplying the highest degree term of 
∏
𝑘
=
1
𝑛
(
𝑥
2
−
𝑘
2
)
∏ 
k=1
n
​
 (x 
2
 −k 
2
 ) by the 
𝑥
x term in 
𝑟
(
𝑥
)
r(x):
[
coefficient of 
𝑥
2
𝑛
]
×
𝐵
𝑥
=
𝑥
2
𝑛
⋅
𝐵
𝑥
=
𝐵
𝑥
2
𝑛
+
1
[coefficient of x 
2n
 ]×Bx=x 
2n
 ⋅Bx=Bx 
2n+1
 
Since there's no 
𝑥
2
𝑛
+
1
x 
2n+1
  term in 
𝐺
(
𝑥
)
G(x), 
𝐵
=
0
B=0.
Constant Term (
𝐶
C):

Evaluate 
𝐺
(
0
)
G(0):
𝐺
(
0
)
=
[
1
+
0
+
0
+
⋯
+
0
]
−
0
=
1
G(0)=[1+0+0+⋯+0]−0=1
On the other hand:
𝐺
(
0
)
=
(
∏
𝑘
=
1
𝑛
(
0
2
−
𝑘
2
)
)
⋅
𝐶
=
(
∏
𝑘
=
1
𝑛
(
−
𝑘
2
)
)
⋅
𝐶
=
(
−
1
)
𝑛
(
𝑛
!
)
2
⋅
𝐶
G(0)=( 
k=1
∏
n
​
 (0 
2
 −k 
2
 ))⋅C=( 
k=1
∏
n
​
 (−k 
2
 ))⋅C=(−1) 
n
 (n!) 
2
 ⋅C
Since 
𝑛
n is even, 
(
−
1
)
𝑛
=
1
(−1) 
n
 =1.
Equate the two expressions:
1
=
(
𝑛
!
)
2
⋅
𝐶
⇒
𝐶
=
1
(
𝑛
!
)
2
1=(n!) 
2
 ⋅C⇒C= 
(n!) 
2
 
1
​
 
Final Form of 
𝑟
(
𝑥
)
r(x):

𝑟
(
𝑥
)
=
−
𝑥
2
+
1
(
𝑛
!
)
2
r(x)=−x 
2
 + 
(n!) 
2
 
1
​
 
Step 6: Expressing 
𝐺
(
𝑥
)
G(x) with Determined Coefficients

Now, substitute the values of 
𝐴
,
𝐵
,
A,B, and 
𝐶
C back into the expression for 
𝐺
(
𝑥
)
G(x):

𝐺
(
𝑥
)
=
(
∏
𝑘
=
1
𝑛
(
𝑥
2
−
𝑘
2
)
)
(
−
𝑥
2
+
1
(
𝑛
!
)
2
)
G(x)=( 
k=1
∏
n
​
 (x 
2
 −k 
2
 ))(−x 
2
 + 
(n!) 
2
 
1
​
 )
Step 7: Solving 
𝐺
(
𝑥
)
=
0
G(x)=0 to Find All Real Solutions

Set 
𝐺
(
𝑥
)
=
0
G(x)=0:

(
∏
𝑘
=
1
𝑛
(
𝑥
2
−
𝑘
2
)
)
(
−
𝑥
2
+
1
(
𝑛
!
)
2
)
=
0
( 
k=1
∏
n
​
 (x 
2
 −k 
2
 ))(−x 
2
 + 
(n!) 
2
 
1
​
 )=0
This equation is satisfied when either:

From the Factored Terms:

(
𝑥
2
−
1
)
(
𝑥
2
−
4
)
⋯
(
𝑥
2
−
𝑛
2
)
=
0
(x 
2
 −1)(x 
2
 −4)⋯(x 
2
 −n 
2
 )=0
This yields roots at:

𝑥
=
±
1
,
±
2
,
…
,
±
𝑛
x=±1,±2,…,±n
These are the roots already provided by the problem's conditions.

From the Quadratic Factor:

−
𝑥
2
+
1
(
𝑛
!
)
2
=
0
⇒
𝑥
2
=
1
(
𝑛
!
)
2
⇒
𝑥
=
±
1
𝑛
!
−x 
2
 + 
(n!) 
2
 
1
​
 =0⇒x 
2
 = 
(n!) 
2
 
1
​
 ⇒x=± 
n!
1
​
 
These are the additional roots arising from the quadratic factor.

Total Real Solutions:

𝑥
=
±
1
,
±
2
,
…
,
±
𝑛
,
±
1
𝑛
!
x=±1,±2,…,±n,± 
n!
1
​
 
Step 8: Verifying the Additional Roots

While the given conditions provided 
2
𝑛
2n roots, the degree of 
𝐺
(
𝑥
)
G(x) is 
2
𝑛
+
2
2n+2, implying two additional roots. Let's ensure these extra roots are valid.

Nature of the Extra Roots:

𝑥
=
±
1
𝑛
!
x=± 
n!
1
​
  are real numbers distinct from the initial 
±
1
,
±
2
,
…
,
±
𝑛
±1,±2,…,±n.
Since 
𝑛
!
≥
2
n!≥2 for 
𝑛
≥
2
n≥2 (and 
𝑛
n is even), 
1
𝑛
!
≤
1
2
n!
1
​
 ≤ 
2
1
​
 , ensuring these roots don't coincide with the initial ones.
Consistency with 
𝑝
(
𝑥
)
p(x):

The polynomial 
𝑝
(
𝑥
)
p(x) was uniquely determined by the 
2
𝑛
2n given conditions.
The additional roots arise from the construction of 
𝐺
(
𝑥
)
G(x) and do not contradict the uniqueness, as 
𝐺
(
𝑥
)
G(x) encapsulates the relationship 
𝑝
(
1
𝑥
)
=
𝑥
2
p( 
x
1
​
 )=x 
2
  beyond the initially provided points.
Conclusion on Extra Roots:

The extra roots are valid and represent additional solutions where 
𝑝
(
1
𝑥
)
=
𝑥
2
p( 
x
1
​
 )=x 
2
 .
These roots are distinct and satisfy the equation independently of the initial conditions.
Final Answer:

The additional real numbers 
𝑥
x satisfying 
𝑝
(
1
𝑥
)
=
𝑥
2
p( 
x
1
​
 )=x 
2
  are:

𝑥
=
±
1
𝑛
!
x=± 
n!
1
​
 
Combined with the given solutions 
𝑥
=
±
1
,
±
2
,
…
,
±
𝑛
x=±1,±2,…,±n, all real numbers satisfying the equation are:

𝑥
=
±
1
,
±
2
,
…
,
±
𝑛
,
±
1
𝑛
!
x=±1,±2,…,±n,± 
n!
1
​
 
Summary of the Approach:

Initial Strategy:

Defined a new function 
𝐹
(
𝑥
)
=
𝑝
(
1
𝑥
)
−
𝑥
2
F(x)=p( 
x
1
​
 )−x 
2
  to encapsulate the condition.
Multiplied by 
𝑥
2
𝑛
x 
2n
  to convert 
𝐹
(
𝑥
)
F(x) into a polynomial 
𝐺
(
𝑥
)
G(x).
Factoring and Determining Coefficients:

Factored 
𝐺
(
𝑥
)
G(x) based on known roots from the given conditions.
Determined the coefficients of the quadratic factor 
𝑟
(
𝑥
)
r(x) by matching leading terms and ensuring polynomial consistency.
Solving for All Real Roots:

Identified both the initial 
2
𝑛
2n roots and the additional 
±
1
𝑛
!
± 
n!
1
​
  roots from the quadratic factor.
Verification:

Ensured that the extra roots are valid and do not interfere with the initial conditions.
Final Conclusion:

Presented the complete set of real solutions, including both the given and additional roots.
Key Takeaways:

Polynomial Construction: By defining a new function that captures the given condition, we transformed the problem into finding the roots of a polynomial, which is a well-understood mathematical process.

Factorization: Leveraging known roots to factor the polynomial simplifies the process of identifying additional roots.

Verification: Always crucial to verify that additional solutions are valid within the context of the original problem.

This systematic approach ensures that all possible solutions are accounted for and that the methodology is robust against potential oversights.






