### Question:
Let $x,y,$ and $z$ be real numbers satisfying the system of equations\begin{align*} xy + 4z &= 60 \\ yz + 4x &= 60 \\ zx + 4y &= 60. \end{align*}Let $S$ be the set of possible values of $x.$ Find the sum of the squares of the elements of $S.$



### Answer:
**First thoughts:**

Hmm, looking at this system of equations:

\[
\begin{cases}
xy + 4z = 60 \quad\quad (1) \\
yz + 4x = 60 \quad\quad (2) \\
zx + 4y = 60 \quad\quad (3)
\end{cases}
\]

I notice that the equations are symmetric in a cyclic way. Each equation involves the product of two variables plus four times the third variable equals 60.

**Brainstorming strategies:**

- **Option 1:** Try to find symmetry or patterns to simplify the system.
- **Option 2:** Express one variable in terms of the others and substitute.
- **Option 3:** Consider special cases, like setting variables equal to each other.

**Exploring Option 1:**

Let's add all three equations to see what happens.

Adding (1), (2), and (3):

\[
(xy + yz + zx) + 4x + 4y + 4z = 180
\]

Let me denote \( P = xy + yz + zx \) and \( S = x + y + z \).

So, we have:

\[
P + 4S = 180 \quad\quad (4)
\]

But this introduces two new variables \( P \) and \( S \), and I'm not sure if this gets me closer to finding \( x \).

**Option 2 seems messy at this point. Maybe Option 3 will be more fruitful.**

**Exploring Option 3: Assume \( x = y = z \):**

Suppose \( x = y = z = k \).

Substituting into equation (1):

\[
k \cdot k + 4k = 60 \\
k^2 + 4k - 60 = 0
\]

Solving the quadratic equation:

\[
k = \frac{-4 \pm \sqrt{(4)^2 - 4 \cdot 1 \cdot (-60)}}{2} \\
k = \frac{-4 \pm \sqrt{16 + 240}}{2} \\
k = \frac{-4 \pm \sqrt{256}}{2} \\
k = \frac{-4 \pm 16}{2}
\]

So, the solutions are:

1. \( k = \frac{-4 + 16}{2} = \frac{12}{2} = 6 \)
2. \( k = \frac{-4 - 16}{2} = \frac{-20}{2} = -10 \)

Thus, \( x = y = z = 6 \) or \( x = y = z = -10 \).

**Possible \( x \) values so far: \( x = 6 \) and \( x = -10 \).**

**Checking for other possibilities:**

Looking back at the equations, perhaps setting one of the variables to 4 might simplify things, since the coefficient 4 appears prominently.

**Suppose \( x = 4 \):**

Substituting \( x = 4 \) into equation (2):

\[
y z + 4 \cdot 4 = 60 \\
y z + 16 = 60 \\
y z = 44 \quad\quad (5)
\]

From equation (1):

\[
4 y + 4 z = 60 \\
4(y + z) = 60 \\
y + z = 15 \quad\quad (6)
\]

Now, we have two equations:

\[
\begin{cases}
y z = 44 \quad\quad (5) \\
y + z = 15 \quad\quad (6)
\end{cases}
\]

This is a classic system to solve for \( y \) and \( z \).

**Solving for \( y \) and \( z \):**

From (6):

\[
z = 15 - y
\]

Substitute into (5):

\[
y(15 - y) = 44 \\
15y - y^2 = 44 \\
-y^2 + 15y - 44 = 0 \\
y^2 - 15y + 44 = 0
\]

Solving the quadratic equation:

\[
y = \frac{15 \pm \sqrt{225 - 176}}{2} \\
y = \frac{15 \pm \sqrt{49}}{2} \\
y = \frac{15 \pm 7}{2}
\]

So, the solutions are:

1. \( y = \frac{15 + 7}{2} = \frac{22}{2} = 11 \)
2. \( y = \frac{15 - 7}{2} = \frac{8}{2} = 4 \)

**Corresponding \( z \) values:**

Using \( z = 15 - y \):

1. When \( y = 11 \), \( z = 15 - 11 = 4 \)
2. When \( y = 4 \), \( z = 15 - 4 = 11 \)

So we have two solutions:

- \( (x, y, z) = (4, 11, 4) \)
- \( (x, y, z) = (4, 4, 11) \)

**Another possible \( x \) value confirmed: \( x = 4 \).**

**Are there any more solutions?**

Let me try another assumption.

**Assume \( y = z \):**

From equations (1) and (2):

\[
\begin{cases}
x y + 4 y = 60 \quad\quad (1a) \\
y^2 + 4 x = 60 \quad\quad (2a)
\end{cases}
\]

From (1a):

\[
x y + 4 y = 60 \\
y(x + 4) = 60 \\
x = \frac{60}{y} - 4 \quad\quad (7)
\]

Substitute \( x \) into (2a):

\[
y^2 + 4 \left( \frac{60}{y} - 4 \right) = 60 \\
y^2 + \left( \frac{240}{y} - 16 \right) = 60 \\
\]

Multiply both sides by \( y \) to eliminate the fraction:

\[
y^3 + 240 - 16 y = 60 y \\
y^3 - 76 y + 240 = 0
\]

**Wait, this cubic equation needs to be solved.**

**Attempting to factor the cubic equation:**

\[
y^3 - 76 y + 240 = 0
\]

Possible rational roots are factors of 240 divided by factors of 1:

\[
\pm1, \pm2, \pm3, \pm4, \pm5, \pm6, \pm8, \pm10, \pm12, \pm15, \pm16, \pm20, \pm24, \pm30, \pm40, \pm60, \pm120, \pm240
\]

Let's test \( y = 4 \):

\[
(4)^3 - 76 \cdot 4 + 240 = 64 - 304 + 240 = 0
\]

So \( y = 4 \) is a root.

**Factor out \( y - 4 \):**

Using polynomial division or synthetic division:

Divide \( y^3 - 76 y + 240 \) by \( y - 4 \):

The result is:

\[
(y - 4)(y^2 + 4 y - 60) = 0
\]

Now, solve \( y^2 + 4 y - 60 = 0 \):

\[
y = \frac{-4 \pm \sqrt{16 + 240}}{2} \\
y = \frac{-4 \pm \sqrt{256}}{2} \\
y = \frac{-4 \pm 16}{2}
\]

So, the solutions are:

1. \( y = \frac{-4 + 16}{2} = \frac{12}{2} = 6 \)
2. \( y = \frac{-4 - 16}{2} = \frac{-20}{2} = -10 \)

**Corresponding \( x \) values:**

Recall from equation (7):

\[
x = \frac{60}{y} - 4
\]

1. When \( y = 4 \):

\[
x = \frac{60}{4} - 4 = 15 - 4 = 11
\]

2. When \( y = 6 \):

\[
x = \frac{60}{6} - 4 = 10 - 4 = 6
\]

3. When \( y = -10 \):

\[
x = \frac{60}{-10} - 4 = -6 - 4 = -10
\]

**Thus, additional \( x \) values are \( x = 11 \) and \( x = -10 \) (which we already had), and \( x = 6 \).**

**Compiling all possible \( x \) values:**

- \( x = -10 \)
- \( x = 4 \)
- \( x = 6 \)
- \( x = 11 \)

**Calculating the sum of the squares of the elements of \( S \):**

\[
(-10)^2 + 4^2 + 6^2 + 11^2 = 100 + 16 + 36 + 121 = 273
\]

**Final Answer:** \(\boxed{273}\)