### Question:
Positive real numbers $b \not= 1$ and $n$ satisfy the equations\[\sqrt{\log_b n} = \log_b \sqrt{n} \qquad \text{and} \qquad b \cdot \log_b n = \log_b (bn).\]The value of $n$ is $\frac{j}{k},$ where $j$ and $k$ are relatively prime positive integers. Find $j+k.$




### Answer:
Alright, let's dive into solving this problem step by step. I'll walk you through my thought process, exploring different strategies, checking for correctness along the way, and adjusting my approach as needed.

**Problem Statement:**
We are given positive real numbers \( b \neq 1 \) and \( n \) that satisfy the following two equations:

1. \( \sqrt{\log_b n} = \log_b \sqrt{n} \)
2. \( b \cdot \log_b n = \log_b (b n) \)

We need to find the value of \( n \) expressed as \( \frac{j}{k} \), where \( j \) and \( k \) are relatively prime positive integers, and then determine \( j + k \).

**First Thoughts:**
When I first look at these equations, I notice that both involve logarithms with base \( b \). The presence of logarithms suggests that properties of logarithms will be crucial in simplifying and solving these equations. Also, since \( b \) is not equal to 1 and both \( b \) and \( n \) are positive real numbers, the logarithms are well-defined.

I also observe that the first equation relates a square root of a logarithm to another logarithm, which might hint at squaring both sides or manipulating the expressions to simplify them. The second equation relates a product involving \( b \) and a logarithm to another logarithmic expression, which might require using logarithmic identities.

**Step 1: Analyze the First Equation**

Let's start with the first equation:

\[
\sqrt{\log_b n} = \log_b \sqrt{n}
\]

**Thought Process:**
I recall that \( \sqrt{x} \) is the same as \( x^{1/2} \). Additionally, \( \sqrt{n} \) can be expressed as \( n^{1/2} \), and there's a logarithmic identity that \( \log_b n^{k} = k \log_b n \).

**Applying Logarithmic Identity:**

\[
\log_b \sqrt{n} = \log_b n^{1/2} = \frac{1}{2} \log_b n
\]

So, the equation becomes:

\[
\sqrt{\log_b n} = \frac{1}{2} \log_b n
\]

**Letâ€™s Set \( x = \log_b n \):**

This substitution simplifies the equation to:

\[
\sqrt{x} = \frac{1}{2} x
\]

**Solving for \( x \):**

Square both sides to eliminate the square root:

\[
(\sqrt{x})^2 = \left(\frac{1}{2} x\right)^2 \\
x = \frac{1}{4} x^2
\]

Rearrange the equation:

\[
x^2 - 4x = 0 \\
x(x - 4) = 0
\]

**Possible Solutions:**

1. \( x = 0 \)
2. \( x = 4 \)

**Checking Validity:**

Since \( x = \log_b n \) and \( b \) is a positive real number not equal to 1, \( \log_b n = 0 \) implies \( n = 1 \). However, substituting \( n = 1 \) into the original equation:

\[
\sqrt{\log_b 1} = \sqrt{0} = 0 \\
\log_b \sqrt{1} = \log_b 1 = 0
\]

This seems valid, but we need to check if it satisfies the second equation as well.

**Hold on a Second:**

Before proceeding, I realize that \( n = 1 \) might be a trivial solution, and the problem likely expects a non-trivial solution. So, let's focus on the second solution \( x = 4 \).

**Step 2: Analyze the Second Equation with \( x = 4 \)**

The second equation is:

\[
b \cdot \log_b n = \log_b (b n)
\]

**Substituting \( x = \log_b n = 4 \):**

\[
b \cdot 4 = \log_b (b n)
\]

**Simplify the Right Side:**

Using logarithmic identities:

\[
\log_b (b n) = \log_b b + \log_b n = 1 + x = 1 + 4 = 5
\]

**Set Up the Equation:**

\[
4b = 5
\]

**Solve for \( b \):**

\[
b = \frac{5}{4}
\]

**Step 3: Find \( n \) Using \( b = \frac{5}{4} \) and \( x = 4 \)**

Recall that \( x = \log_b n = 4 \). We can express \( n \) in terms of \( b \):

\[
n = b^x = \left(\frac{5}{4}\right)^4
\]

**Calculate \( \left(\frac{5}{4}\right)^4 \):**

\[
\left(\frac{5}{4}\right)^4 = \frac{5^4}{4^4} = \frac{625}{256}
\]

**Step 4: Verify the Solution**

Let's ensure that both original equations are satisfied with \( b = \frac{5}{4} \) and \( n = \frac{625}{256} \).

1. **First Equation:**

\[
\sqrt{\log_b n} = \sqrt{4} = 2 \\
\log_b \sqrt{n} = \log_b \left(\frac{625}{256}\right)^{1/2} = \log_b \left(\frac{25}{16}\right) = \frac{1}{2} \log_b \left(\frac{625}{256}\right) = \frac{1}{2} \cdot 4 = 2
\]

Both sides equal 2, so the first equation holds.

2. **Second Equation:**

\[
b \cdot \log_b n = \frac{5}{4} \cdot 4 = 5 \\
\log_b (b n) = \log_b \left(\frac{5}{4} \cdot \frac{625}{256}\right) = \log_b \left(\frac{3125}{1024}\right) = \log_b \left(\left(\frac{5}{4}\right)^5\right) = 5 \log_b \left(\frac{5}{4}\right) = 5 \cdot 1 = 5
\]

Both sides equal 5, so the second equation also holds.

**Conclusion:**

We've found that \( n = \frac{625}{256} \). The problem asks for \( j + k \) where \( n = \frac{j}{k} \) and \( j \) and \( k \) are relatively prime positive integers.

Here, \( j = 625 \) and \( k = 256 \). Since 625 and 256 share no common factors other than 1, they are relatively prime.

\[
j + k = 625 + 256 = 881
\]

**Final Answer:**

\(\boxed{881}\)