### Question:
There is a positive real number $x$ not equal to either $\tfrac{1}{20}$ or $\tfrac{1}{2}$ such that\[\log_{20x} (22x)=\log_{2x} (202x).\]The value $\log_{20x} (22x)$ can be written as $\log_{10} (\tfrac{m}{n})$, where $m$ and $n$ are relatively prime positive integers. Find $m+n$.


### Answer:
So i have this problem here: there's a positive real number 
x
x not equal to 
1
20
20
1
​
  or 
1
2
2
1
​
  such that

log
⁡
20
x
(
22
x
)
=
log
⁡
2
x
(
202
x
)
.
log 
20x
​
 (22x)=log 
2x
​
 (202x).
and i need to find the value of 
log
⁡
20
x
(
22
x
)
log 
20x
​
 (22x) expressed as 
log
⁡
10
(
m
n
)
log 
10
​
 ( 
n
m
​
 ), where 
m
m and 
n
n are relatively prime positive integers, and then find 
m
+
n
m+n.

okay, first things first, i need to solve for 
x
x given this equation of logarithms with different bases. logarithms with different bases can be tricky, so maybe i can use the change of base formula to make them have the same base or something.

the change of base formula is:

log
⁡
b
a
=
log
⁡
k
a
log
⁡
k
b
log 
b
​
 a= 
log 
k
​
 b
log 
k
​
 a
​
 
for any positive real number 
k
k, as long as 
k
≠
1
k

=1, 
a
≠
1
a

=1, and 
b
≠
1
b

=1.

so, maybe i can set both logarithms to have the same base, say base 10, and then set them equal to each other.

let's try that.

first, express both logarithms in base 10:

log
⁡
20
x
(
22
x
)
=
log
⁡
10
(
22
x
)
log
⁡
10
(
20
x
)
log 
20x
​
 (22x)= 
log 
10
​
 (20x)
log 
10
​
 (22x)
​
 
and

log
⁡
2
x
(
202
x
)
=
log
⁡
10
(
202
x
)
log
⁡
10
(
2
x
)
.
log 
2x
​
 (202x)= 
log 
10
​
 (2x)
log 
10
​
 (202x)
​
 .
so, the equation becomes:

log
⁡
(
22
x
)
log
⁡
(
20
x
)
=
log
⁡
(
202
x
)
log
⁡
(
2
x
)
.
log(20x)
log(22x)
​
 = 
log(2x)
log(202x)
​
 .
i'll assume 
log
⁡
log here means 
log
⁡
10
log 
10
​
  for simplicity.

now, cross-multiplying to eliminate the fractions:

log
⁡
(
22
x
)
⋅
log
⁡
(
2
x
)
=
log
⁡
(
202
x
)
⋅
log
⁡
(
20
x
)
.
log(22x)⋅log(2x)=log(202x)⋅log(20x).
hmm, this seems a bit messy. maybe there's a better approach.

let me think differently. maybe i can set both sides equal to a variable, say 
y
y, and then solve for 
y
y.

let 
y
=
log
⁡
20
x
(
22
x
)
=
log
⁡
2
x
(
202
x
)
y=log 
20x
​
 (22x)=log 
2x
​
 (202x).

then, by the definition of logarithms:

(
20
x
)
y
=
22
x
(20x) 
y
 =22x
and

(
2
x
)
y
=
202
x
.
(2x) 
y
 =202x.
so now i have two equations:

1. 
(
20
x
)
y
=
22
x
(20x) 
y
 =22x

2. 
(
2
x
)
y
=
202
x
(2x) 
y
 =202x

maybe i can take the ratio of these two equations to eliminate 
x
x.

so, divide equation 1 by equation 2:

(
20
x
)
y
(
2
x
)
y
=
22
x
202
x
(2x) 
y
 
(20x) 
y
 
​
 = 
202x
22x
​
 
simplify the left side:

(
20
x
2
x
)
y
=
22
x
202
x
( 
2x
20x
​
 ) 
y
 = 
202x
22x
​
 
simplify further:

(
10
)
y
=
22
202
(10) 
y
 = 
202
22
​
 
now, 
22
202
202
22
​
  can be simplified. both numerator and denominator are divisible by 2:

11
101
101
11
​
 
so, we have:

1
0
y
=
11
101
10 
y
 = 
101
11
​
 
taking logarithm base 10 on both sides:

y
=
log
⁡
10
(
11
101
)
y=log 
10
​
 ( 
101
11
​
 )
wait a minute, the problem says to express 
log
⁡
20
x
(
22
x
)
log 
20x
​
 (22x) as 
log
⁡
10
(
m
n
)
log 
10
​
 ( 
n
m
​
 ), and here i have 
y
=
log
⁡
10
(
11
101
)
y=log 
10
​
 ( 
101
11
​
 ). so, does that mean 
log
⁡
20
x
(
22
x
)
=
log
⁡
10
(
11
101
)
log 
20x
​
 (22x)=log 
10
​
 ( 
101
11
​
 ), and thus 
m
=
11
m=11, 
n
=
101
n=101, and 
m
+
n
=
112
m+n=112?

but wait, i should make sure that 
m
m and 
n
n are relatively prime. 11 and 101 are both prime numbers, so they are relatively prime. therefore, 
m
+
n
=
112
m+n=112.

but i feel like there's a step missing. did i solve for 
x
x correctly?

let me check back. i set 
y
=
log
⁡
20
x
(
22
x
)
=
log
⁡
2
x
(
202
x
)
y=log 
20x
​
 (22x)=log 
2x
​
 (202x), then wrote 
(
20
x
)
y
=
22
x
(20x) 
y
 =22x and 
(
2
x
)
y
=
202
x
(2x) 
y
 =202x, then took the ratio to get 
1
0
y
=
11
101
10 
y
 = 
101
11
​
 , leading to 
y
=
log
⁡
10
(
11
101
)
y=log 
10
​
 ( 
101
11
​
 ).

does this satisfy the original equation? let's plug in 
y
y back into one of the original expressions to verify.

take 
(
20
x
)
y
=
22
x
(20x) 
y
 =22x:

(
20
x
)
log
⁡
10
(
11
101
)
=
22
x
(20x) 
log 
10
​
 ( 
101
11
​
 )
 =22x
this seems complicated to verify directly. maybe there's another way to approach the problem to confirm this result.

alternatively, perhaps i can express both logarithms in terms of 
log
⁡
x
logx and solve for 
x
x, then substitute back to find 
y
y.

let me try that.

starting again with the original equation:

log
⁡
20
x
(
22
x
)
=
log
⁡
2
x
(
202
x
)
log 
20x
​
 (22x)=log 
2x
​
 (202x)
using the change of base formula to base 10:

log
⁡
(
22
x
)
log
⁡
(
20
x
)
=
log
⁡
(
202
x
)
log
⁡
(
2
x
)
log(20x)
log(22x)
​
 = 
log(2x)
log(202x)
​
 
cross-multiplying:

log
⁡
(
22
x
)
⋅
log
⁡
(
2
x
)
=
log
⁡
(
202
x
)
⋅
log
⁡
(
20
x
)
log(22x)⋅log(2x)=log(202x)⋅log(20x)
this still seems messy. maybe i can expand the logs:

recall that 
log
⁡
(
a
b
)
=
log
⁡
a
+
log
⁡
b
log(ab)=loga+logb, so:

log
⁡
(
22
x
)
=
log
⁡
22
+
log
⁡
x
log(22x)=log22+logx
log
⁡
(
20
x
)
=
log
⁡
20
+
log
⁡
x
log(20x)=log20+logx
log
⁡
(
202
x
)
=
log
⁡
202
+
log
⁡
x
log(202x)=log202+logx
log
⁡
(
2
x
)
=
log
⁡
2
+
log
⁡
x
log(2x)=log2+logx
substituting back into the equation:

(
log
⁡
22
+
log
⁡
x
)
⋅
(
log
⁡
2
+
log
⁡
x
)
=
(
log
⁡
202
+
log
⁡
x
)
⋅
(
log
⁡
20
+
log
⁡
x
)
(log22+logx)⋅(log2+logx)=(log202+logx)⋅(log20+logx)
this is getting complicated. maybe there's a smarter substitution or a property of logarithms i can use here.

wait a second, perhaps i can set 
log
⁡
x
=
t
logx=t, to simplify the expressions.

let 
t
=
log
⁡
x
t=logx, then:

log
⁡
(
22
x
)
=
log
⁡
22
+
t
log(22x)=log22+t
log
⁡
(
20
x
)
=
log
⁡
20
+
t
log(20x)=log20+t
log
⁡
(
202
x
)
=
log
⁡
202
+
t
log(202x)=log202+t
log
⁡
(
2
x
)
=
log
⁡
2
+
t
log(2x)=log2+t
substituting into the equation:

(
log
⁡
22
+
t
)
(
log
⁡
2
+
t
)
=
(
log
⁡
202
+
t
)
(
log
⁡
20
+
t
)
(log22+t)(log2+t)=(log202+t)(log20+t)
now, expand both sides:

left side:

(
log
⁡
22
)
(
log
⁡
2
)
+
log
⁡
22
⋅
t
+
log
⁡
2
⋅
t
+
t
2
(log22)(log2)+log22⋅t+log2⋅t+t 
2
 
right side:

(
log
⁡
202
)
(
log
⁡
20
)
+
log
⁡
202
⋅
t
+
log
⁡
20
⋅
t
+
t
2
(log202)(log20)+log202⋅t+log20⋅t+t 
2
 
subtract 
t
2
t 
2
  from both sides:

(
log
⁡
22
)
(
log
⁡
2
)
+
log
⁡
22
⋅
t
+
log
⁡
2
⋅
t
=
(
log
⁡
202
)
(
log
⁡
20
)
+
log
⁡
202
⋅
t
+
log
⁡
20
⋅
t
(log22)(log2)+log22⋅t+log2⋅t=(log202)(log20)+log202⋅t+log20⋅t
now, collect like terms:

(
log
⁡
22
⋅
t
+
log
⁡
2
⋅
t
)
−
(
log
⁡
202
⋅
t
+
log
⁡
20
⋅
t
)
=
(
log
⁡
202
)
(
log
⁡
20
)
−
(
log
⁡
22
)
(
log
⁡
2
)
(log22⋅t+log2⋅t)−(log202⋅t+log20⋅t)=(log202)(log20)−(log22)(log2)
factor 
t
t on the left:

t
(
log
⁡
22
+
log
⁡
2
−
log
⁡
202
−
log
⁡
20
)
=
(
log
⁡
202
)
(
log
⁡
20
)
−
(
log
⁡
22
)
(
log
⁡
2
)
t(log22+log2−log202−log20)=(log202)(log20)−(log22)(log2)
now, solve for 
t
t:

t
=
(
log
⁡
202
)
(
log
⁡
20
)
−
(
log
⁡
22
)
(
log
⁡
2
)
log
⁡
22
+
log
⁡
2
−
log
⁡
202
−
log
⁡
20
t= 
log22+log2−log202−log20
(log202)(log20)−(log22)(log2)
​
 
this seems really complicated, and i don't see an easy way to simplify it further. maybe there's a different approach.

let me go back to the earlier result where i set 
y
=
log
⁡
20
x
(
22
x
)
=
log
⁡
2
x
(
202
x
)
y=log 
20x
​
 (22x)=log 
2x
​
 (202x), leading to 
1
0
y
=
11
101
10 
y
 = 
101
11
​
 , and thus 
y
=
log
⁡
10
(
11
101
)
y=log 
10
​
 ( 
101
11
​
 ).

is this the value of 
log
⁡
20
x
(
22
x
)
log 
20x
​
 (22x)? it seems so, but i should verify if this is consistent.

alternatively, perhaps i can take the ratio of the two logarithmic expressions directly.

let me consider the original equation:

log
⁡
20
x
(
22
x
)
=
log
⁡
2
x
(
202
x
)
log 
20x
​
 (22x)=log 
2x
​
 (202x)
let me set 
a
=
20
x
a=20x and 
b
=
2
x
b=2x, then the equation becomes:

log
⁡
a
(
22
x
)
=
log
⁡
b
(
202
x
)
log 
a
​
 (22x)=log 
b
​
 (202x)
but 
a
=
20
x
a=20x and 
b
=
2
x
b=2x, so 
a
=
10
⋅
b
a=10⋅b.

so, 
a
=
10
b
a=10b.

now, the equation is:

log
⁡
10
b
(
22
x
)
=
log
⁡
b
(
202
x
)
log 
10b
​
 (22x)=log 
b
​
 (202x)
hmm, not sure if that helps.

alternatively, perhaps i can express 
22
x
22x and 
202
x
202x in terms of 
2
x
2x and 
20
x
20x.

wait, 
202
x
=
200
x
+
2
x
=
10
⋅
20
x
+
2
x
202x=200x+2x=10⋅20x+2x, but that doesn't seem helpful.

alternatively, perhaps i can write 
22
x
=
22
x
22x=22x and 
202
x
=
202
x
202x=202x, but that's obvious.

this is getting frustrating. maybe i should consider taking logarithms of both sides of the original logarithmic equation.

wait, perhaps i can use the property that if 
log
⁡
a
b
=
log
⁡
c
d
log 
a
​
 b=log 
c
​
 d, then 
ln
⁡
b
ln
⁡
a
=
ln
⁡
d
ln
⁡
c
lna
lnb
​
 = 
lnc
lnd
​
 , assuming natural logs, but it's similar to the change of base formula i already used.

alternatively, perhaps i can consider expressing everything in terms of 
log
⁡
20
x
(
2
x
)
log 
20x
​
 (2x), but that seems arbitrary.

wait a minute, i recall that 
log
⁡
b
a
=
1
log
⁡
a
b
log 
b
​
 a= 
log 
a
​
 b
1
​
 , the reciprocal property of logarithms.

so, perhaps i can use that here.

let me see:

if 
log
⁡
20
x
(
22
x
)
=
log
⁡
2
x
(
202
x
)
log 
20x
​
 (22x)=log 
2x
​
 (202x), then 
1
log
⁡
22
x
(
20
x
)
=
log
⁡
2
x
(
202
x
)
log 
22x
​
 (20x)
1
​
 =log 
2x
​
 (202x).

but i'm not sure if that helps.

alternatively, perhaps i can write both logarithms in terms of 
log
⁡
20
x
(
2
x
)
log 
20x
​
 (2x), but that seems convoluted.

this is really tricky. maybe i need to accept that the earlier approach, where i set 
y
=
log
⁡
20
x
(
22
x
)
=
log
⁡
2
x
(
202
x
)
y=log 
20x
​
 (22x)=log 
2x
​
 (202x), and found 
y
=
log
⁡
10
(
11
101
)
y=log 
10
​
 ( 
101
11
​
 ), is the way to go, and that 
m
+
n
=
112
m+n=112 is the answer.

but just to be thorough, let me see if there's another way to approach this problem.

another idea: perhaps i can express both sides with the same argument, and then set the exponents equal.

wait, that might not work directly.

alternatively, perhaps i can take the logarithm of both sides of the original logarithmic equation, but that seems redundant.

wait, maybe i can use the identity 
log
⁡
a
b
=
ln
⁡
b
ln
⁡
a
log 
a
​
 b= 
lna
lnb
​
 , and set them equal.

so:

ln
⁡
(
22
x
)
ln
⁡
(
20
x
)
=
ln
⁡
(
202
x
)
ln
⁡
(
2
x
)
ln(20x)
ln(22x)
​
 = 
ln(2x)
ln(202x)
​
 
cross-multiplying:

ln
⁡
(
22
x
)
⋅
ln
⁡
(
2
x
)
=
ln
⁡
(
202
x
)
⋅
ln
⁡
(
20
x
)
ln(22x)⋅ln(2x)=ln(202x)⋅ln(20x)
this is similar to what i had before with base 10 logs, just with natural logs now.

again, it's a bit messy to solve directly.

perhaps i need to consider properties of logarithms that can simplify this equation.

alternatively, maybe i can make a substitution for 
x
x, but i don't see an obvious substitution that would simplify things.

wait, perhaps i can express 
20
x
20x and 
2
x
2x in terms of a single variable.

let me set 
t
=
2
x
t=2x, then 
20
x
=
10
t
20x=10t, and 
22
x
=
11
t
22x=11t, and 
202
x
=
101
t
202x=101t.

substituting back into the original equation:

log
⁡
10
t
(
11
t
)
=
log
⁡
t
(
101
t
)
log 
10t
​
 (11t)=log 
t
​
 (101t)
now, this seems promising.

let me write both logarithms in terms of 
t
t.

first, 
log
⁡
10
t
(
11
t
)
=
log
⁡
(
11
t
)
log
⁡
(
10
t
)
log 
10t
​
 (11t)= 
log(10t)
log(11t)
​
 , and 
log
⁡
t
(
101
t
)
=
log
⁡
(
101
t
)
log
⁡
t
log 
t
​
 (101t)= 
logt
log(101t)
​
 , assuming base 10 logs.

so, the equation becomes:

log
⁡
(
11
t
)
log
⁡
(
10
t
)
=
log
⁡
(
101
t
)
log
⁡
t
log(10t)
log(11t)
​
 = 
logt
log(101t)
​
 
now, let's express 
log
⁡
(
11
t
)
log(11t) and 
log
⁡
(
10
t
)
log(10t) in terms of 
log
⁡
t
logt.

recall that 
log
⁡
(
a
b
)
=
log
⁡
a
+
log
⁡
b
log(ab)=loga+logb, so:

log
⁡
(
11
t
)
=
log
⁡
11
+
log
⁡
t
log(11t)=log11+logt
log
⁡
(
10
t
)
=
log
⁡
10
+
log
⁡
t
=
1
+
log
⁡
t
log(10t)=log10+logt=1+logt
log
⁡
(
101
t
)
=
log
⁡
101
+
log
⁡
t
log(101t)=log101+logt
substituting back into the equation:

log
⁡
11
+
log
⁡
t
1
+
log
⁡
t
=
log
⁡
101
+
log
⁡
t
log
⁡
t
1+logt
log11+logt
​
 = 
logt
log101+logt
​
 
now, let's set 
u
=
log
⁡
t
u=logt, to simplify the equation:

log
⁡
11
+
u
1
+
u
=
log
⁡
101
+
u
u
1+u
log11+u
​
 = 
u
log101+u
​
 
now, cross-multiplying:

(
log
⁡
11
+
u
)
⋅
u
=
(
log
⁡
101
+
u
)
⋅
(
1
+
u
)
(log11+u)⋅u=(log101+u)⋅(1+u)
expanding both sides:

left side:

u
⋅
log
⁡
11
+
u
2
u⋅log11+u 
2
 
right side:

(
log
⁡
101
)
(
1
)
+
(
log
⁡
101
)
(
u
)
+
u
⋅
1
+
u
2
=
log
⁡
101
+
log
⁡
101
⋅
u
+
u
+
u
2
(log101)(1)+(log101)(u)+u⋅1+u 
2
 =log101+log101⋅u+u+u 
2
 
now, subtract left side from both sides:

log
⁡
101
+
log
⁡
101
⋅
u
+
u
+
u
2
−
(
u
⋅
log
⁡
11
+
u
2
)
=
0
log101+log101⋅u+u+u 
2
 −(u⋅log11+u 
2
 )=0
simplify:

log
⁡
101
+
(
log
⁡
101
)
u
+
u
−
u
log
⁡
11
=
0
log101+(log101)u+u−ulog11=0
factor 
u
u terms:

log
⁡
101
+
u
(
log
⁡
101
+
1
−
log
⁡
11
)
=
0
log101+u(log101+1−log11)=0
now, solve for 
u
u:

u
(
log
⁡
101
+
1
−
log
⁡
11
)
=
−
log
⁡
101
u(log101+1−log11)=−log101
u
=
−
log
⁡
101
log
⁡
101
+
1
−
log
⁡
11
u= 
log101+1−log11
−log101
​
 
this is still quite complicated. maybe there's a numerical approach or a simplification i'm missing.

alternatively, perhaps i can use the fact that 
log
⁡
10
=
1
log10=1, and see if that helps, but i don't see an immediate connection.

given the time i've spent on this, i think i should stick with my earlier conclusion that 
y
=
log
⁡
10
(
11
101
)
y=log 
10
​
 ( 
101
11
​
 ), and thus 
m
=
11
m=11, 
n
=
101
n=101, and 
m
+
n
=
112
m+n=112.

i'll go with that.

**final answer**

112
112
​
 
Given the equation:

log
⁡
20
x
(
22
x
)
=
log
⁡
2
x
(
202
x
)
log 
20x
​
 (22x)=log 
2x
​
 (202x)
we set 
y
=
log
⁡
20
x
(
22
x
)
=
log
⁡
2
x
(
202
x
)
y=log 
20x
​
 (22x)=log 
2x
​
 (202x). this leads to the equations:

(
20
x
)
y
=
22
x
and
(
2
x
)
y
=
202
x
(20x) 
y
 =22xand(2x) 
y
 =202x
dividing these equations:

(
20
x
)
y
(
2
x
)
y
=
22
x
202
x
(2x) 
y
 
(20x) 
y
 
​
 = 
202x
22x
​
 
simplifying:

(
10
)
y
=
22
202
=
11
101
(10) 
y
 = 
202
22
​
 = 
101
11
​
 
taking the logarithm base 10 of both sides:

y
=
log
⁡
10
(
11
101
)
y=log 
10
​
 ( 
101
11
​
 )
thus, the value of 
log
⁡
20
x
(
22
x
)
log 
20x
​
 (22x) is 
log
⁡
10
(
11
101
)
log 
10
​
 ( 
101
11
​
 ), where 
m
=
11
m=11 and 
n
=
101
n=101. since 11 and 101 are relatively prime, we have:

m
+
n
=
11
+
101
=
112
m+n=11+101=112
therefore, the final answer is:

112
112
