### Question:

Quadratic polynomials $P(x)$ and $Q(x)$ have leading coefficients $2$ and $-2,$ respectively. The graphs of both polynomials pass through the two points $(16,54)$ and $(20,53).$ Find $P(0) + Q(0).$

### Answer:

Alright, let's tackle this problem step by step, thinking through each part carefully to ensure we arrive at the correct solution. Here's the problem again for reference:

**Problem:**  
Quadratic polynomials \( P(x) \) and \( Q(x) \) have leading coefficients \( 2 \) and \( -2 \), respectively. The graphs of both polynomials pass through the two points \( (16,54) \) and \( (20,53) \). Find \( P(0) + Q(0) \).

---

### **Initial Thoughts and Strategy**

When dealing with quadratic polynomials, especially when given specific points they pass through, it's natural to think about expressing the polynomials in their standard form and setting up equations based on the given points. 

Given that both polynomials pass through the same two points, we can leverage this to set up a system of equations for each polynomial. Once we have the coefficients, finding \( P(0) + Q(0) \) (which are essentially the constant terms of each polynomial) should be straightforward.

But before diving in, let's outline the steps:

1. **Express \( P(x) \) and \( Q(x) \) in standard quadratic form.**
2. **Use the given points to set up equations for each polynomial.**
3. **Solve the resulting systems to find the coefficients.**
4. **Compute \( P(0) + Q(0) \).**

Let's proceed with this plan, keeping an eye out for any inconsistencies or easier methods that might present themselves along the way.

---

### **Step 1: Expressing the Polynomials**

Given the leading coefficients, we can write the polynomials as:

- \( P(x) = 2x^2 + bx + c \)
- \( Q(x) = -2x^2 + dx + e \)

Here, \( b \) and \( c \) are the coefficients we need to find for \( P(x) \), and \( d \) and \( e \) for \( Q(x) \).

**Reflection:**  
This seems straightforward. By knowing the leading coefficients, we reduce the number of unknowns, making the system of equations easier to handle.

---

### **Step 2: Setting Up Equations Using Given Points**

Both polynomials pass through \( (16,54) \) and \( (20,53) \). Let's plug these into each polynomial.

#### **For \( P(x) \):**

1. **At \( x = 16 \):**
   \[
   2(16)^2 + 16b + c = 54 \\
   512 + 16b + c = 54 \quad \text{(Equation 1)}
   \]

2. **At \( x = 20 \):**
   \[
   2(20)^2 + 20b + c = 53 \\
   800 + 20b + c = 53 \quad \text{(Equation 2)}
   \]

#### **For \( Q(x) \):**

1. **At \( x = 16 \):**
   \[
   -2(16)^2 + 16d + e = 54 \\
   -512 + 16d + e = 54 \quad \text{(Equation 3)}
   \]

2. **At \( x = 20 \):**
   \[
   -2(20)^2 + 20d + e = 53 \\
   -800 + 20d + e = 53 \quad \text{(Equation 4)}
   \]

**Reflection:**  
Now we have four equations with four unknowns. Solving them systematically should yield the coefficients we're after. It's essential to ensure calculations are accurate here to avoid compounding errors later.

---

### **Step 3: Solving for Coefficients**

Let's tackle \( P(x) \) first.

#### **Solving for \( P(x) \):**

We have:
- Equation 1: \( 512 + 16b + c = 54 \)
- Equation 2: \( 800 + 20b + c = 53 \)

**Subtract Equation 1 from Equation 2:**
\[
(800 - 512) + (20b - 16b) + (c - c) = 53 - 54 \\
288 + 4b = -1
\]
\[
4b = -1 - 288 \\
4b = -289 \\
b = -\frac{289}{4}
\]

**Reflection:**  
The value of \( b \) is a fractional negative number. It might seem cumbersome, but fractional coefficients are common in polynomial problems, especially when dealing with specific points.

**Now, substitute \( b \) back into Equation 1 to find \( c \):**
\[
512 + 16\left(-\frac{289}{4}\right) + c = 54 \\
512 - 4 \times 289 + c = 54 \\
512 - 1156 + c = 54 \\
-644 + c = 54 \\
c = 54 + 644 \\
c = 698
\]

#### **Solving for \( Q(x) \):**

We have:
- Equation 3: \( -512 + 16d + e = 54 \)
- Equation 4: \( -800 + 20d + e = 53 \)

**Subtract Equation 3 from Equation 4:**
\[
(-800 + 512) + (20d - 16d) + (e - e) = 53 - 54 \\
-288 + 4d = -1
\]
\[
4d = -1 + 288 \\
4d = 287 \\
d = \frac{287}{4}
\]

**Reflection:**  
Similar to \( b \), \( d \) is also a fractional value but positive this time. Itâ€™s interesting to see how the coefficients differ between \( P(x) \) and \( Q(x) \), reflecting their leading coefficients' signs.

**Now, substitute \( d \) back into Equation 3 to find \( e \):**
\[
-512 + 16\left(\frac{287}{4}\right) + e = 54 \\
-512 + 4 \times 287 + e = 54 \\
-512 + 1148 + e = 54 \\
636 + e = 54 \\
e = 54 - 636 \\
e = -582
\]

**Reflection:**  
The constant term \( e \) is negative, which balances out the negative leading coefficient in \( Q(x) \). The calculations seem consistent so far.

---

### **Step 4: Computing \( P(0) + Q(0) \)**

Recall that for any polynomial \( R(x) = ax^2 + bx + c \), the value \( R(0) = c \). Therefore:

\[
P(0) = c = 698 \\
Q(0) = e = -582 \\
\]

\[
P(0) + Q(0) = 698 + (-582) = 116
\]

**Final Check:**  
Let's briefly verify if the coefficients make sense by plugging them back into one of the original equations.

**For \( P(x) \) at \( x = 16 \):**
\[
2(16)^2 + (-\frac{289}{4})(16) + 698 \\
= 512 - \frac{289}{4} \times 16 + 698 \\
= 512 - 1156 + 698 \\
= 54 \quad \text{(matches the given point)}
\]

**For \( Q(x) \) at \( x = 20 \):**
\[
-2(20)^2 + \frac{287}{4}(20) - 582 \\
= -800 + \frac{287}{4} \times 20 - 582 \\
= -800 + 1435 - 582 \\
= 53 \quad \text{(matches the given point)}
\]

**Reflection:**  
Both checks align perfectly with the given points, confirming the correctness of our coefficients and the final answer.

---

### **Conclusion**

After systematically setting up and solving the equations derived from the given points, we've determined that:

\[
P(0) + Q(0) = \boxed{116}
\]