### Question:
Positive real numbers $b \not= 1$ and $n$ satisfy the equations\[\sqrt{\log_b n} = \log_b \sqrt{n} \qquad \text{and} \qquad b \cdot \log_b n = \log_b (bn).\]The value of $n$ is $\frac{j}{k},$ where $j$ and $k$ are relatively prime positive integers. Find $j+k.$



### Answer:

Sure, let's tackle this problem step by step, exploring different strategies and reflecting on each approach to ensure we're on the right track. Here's how I would approach solving it:

---

**Problem Statement:**

Positive real numbers \( b \neq 1 \) and \( n \) satisfy the equations
\[
\sqrt{\log_b n} = \log_b \sqrt{n} \quad \text{and} \quad b \cdot \log_b n = \log_b (bn).
\]
Find the value of \( n \) expressed as \( \frac{j}{k} \), where \( j \) and \( k \) are relatively prime positive integers. Then, compute \( j + k \).

---

**Brainstorming and Strategy Exploration:**

To solve for \( n \), we have two equations involving logarithms with base \( b \). Given that \( b \neq 1 \) and both \( b \) and \( n \) are positive real numbers, we can utilize logarithmic identities and properties to simplify and solve the equations.

Possible strategies include:

1. **Simplify Each Equation Separately:** Attempt to express \( n \) in terms of \( b \) by manipulating each equation independently.

2. **Express \( b \) in Terms of \( n \):** Try to find a relationship where \( b \) is expressed as a function of \( n \), then substitute back into one of the equations.

3. **Use Logarithmic Identities:** Apply properties of logarithms to simplify expressions and possibly set up an equation that can be solved for \( n \).

4. **Set Up a System of Equations:** Treat the two given equations as a system and solve them simultaneously for \( b \) and \( n \).

Given the structure of the problem, the most straightforward approach seems to be simplifying each equation using logarithmic properties and then solving the resulting system. Let's proceed with this method.

---

**First Equation Analysis:**

\[
\sqrt{\log_b n} = \log_b \sqrt{n}
\]

*Objective:* Simplify this equation to find a relationship between \( \log_b n \) and \( n \).

**Step 1:** Recall that \( \log_b \sqrt{n} \) can be rewritten using logarithmic identities.

\[
\log_b \sqrt{n} = \log_b n^{1/2} = \frac{1}{2} \log_b n
\]

So, the equation becomes:

\[
\sqrt{\log_b n} = \frac{1}{2} \log_b n
\]

**Step 2:** Let’s introduce a substitution to simplify the equation. Let \( x = \log_b n \). Then, the equation becomes:

\[
\sqrt{x} = \frac{1}{2} x
\]

**Step 3:** Square both sides to eliminate the square root:

\[
(\sqrt{x})^2 = \left(\frac{1}{2} x\right)^2 \implies x = \frac{1}{4} x^2
\]

**Step 4:** Rearrange the equation to form a quadratic equation:

\[
\frac{1}{4} x^2 - x = 0 \implies x^2 - 4x = 0
\]

**Step 5:** Factor the quadratic equation:

\[
x(x - 4) = 0
\]

**Step 6:** Solve for \( x \):

\[
x = 0 \quad \text{or} \quad x = 4
\]

**Step 7:** Recall that \( x = \log_b n \), so:

- If \( x = 0 \), then \( \log_b n = 0 \implies n = b^0 = 1 \).
- If \( x = 4 \), then \( \log_b n = 4 \implies n = b^4 \).

**Reflection:** We've found two potential solutions for \( n \) from the first equation: \( n = 1 \) or \( n = b^4 \). However, we need to verify which of these (if any) satisfy the second equation. It’s possible that one of these might not satisfy both equations simultaneously.

---

**Second Equation Analysis:**

\[
b \cdot \log_b n = \log_b (bn)
\]

*Objective:* Use the solutions from the first equation to determine the correct value of \( n \) and find \( b \).

**Step 1:** Consider the two cases obtained from the first equation.

**Case 1:** \( n = 1 \)

- Left Side (LS):

\[
b \cdot \log_b 1 = b \cdot 0 = 0
\]

- Right Side (RS):

\[
\log_b (b \cdot 1) = \log_b b = 1
\]

- Comparison:

\[
0 \neq 1
\]

**Conclusion for Case 1:** \( n = 1 \) does not satisfy the second equation. Therefore, \( n = 1 \) is not a valid solution.

**Case 2:** \( n = b^4 \)

- Left Side (LS):

\[
b \cdot \log_b b^4 = b \cdot 4 = 4b
\]

- Right Side (RS):

\[
\log_b (b \cdot b^4) = \log_b b^5 = 5
\]

- Comparison:

\[
4b = 5
\]

**Step 2:** Solve for \( b \):

\[
4b = 5 \implies b = \frac{5}{4}
\]

**Step 3:** Now that we have \( b = \frac{5}{4} \), substitute back into \( n = b^4 \):

\[
n = \left(\frac{5}{4}\right)^4
\]

**Step 4:** Calculate \( \left(\frac{5}{4}\right)^4 \):

\[
\left(\frac{5}{4}\right)^4 = \frac{5^4}{4^4} = \frac{625}{256}
\]

**Reflection:** We’ve determined that \( n = \frac{625}{256} \) when \( b = \frac{5}{4} \). This solution satisfies both original equations:

- For the first equation:

\[
\sqrt{\log_{\frac{5}{4}} \left(\frac{625}{256}\right)} = \sqrt{4} = 2
\]
\[
\log_{\frac{5}{4}} \sqrt{\frac{625}{256}} = \log_{\frac{5}{4}} \left(\frac{25}{16}\right) = 2
\]
Thus, both sides are equal.

- For the second equation:

\[
b \cdot \log_b n = \frac{5}{4} \cdot 4 = 5
\]
\[
\log_b (bn) = \log_{\frac{5}{4}} \left(\frac{5}{4} \cdot \frac{625}{256}\right) = \log_{\frac{5}{4}} \left(\frac{3125}{1024}\right) = 5
\]
Again, both sides are equal.

Since both equations are satisfied, \( n = \frac{625}{256} \) is indeed the correct solution.

---

**Final Calculation:**

Given \( n = \frac{625}{256} \), where \( j = 625 \) and \( k = 256 \), which are relatively prime.

Thus,

\[
j + k = 625 + 256 = 881
\]

**Answer:** \(\boxed{881}\)